src/program_proof/session/session_definitions.v
@@ -1,14 +1,21 @@
 From Perennial.program_proof.session Require Export session_prelude.
+From Goose.session Require server client.
+
+Module SessionServer := Goose.session.server.
+Module SessionClient := Goose.session.client.
 
 #[local] Tactic Notation "tac_val_t" :=
   let val := lazymatch goal with [ |- val_ty (?val _) _ ] => val end in
-  lazymatch goal with [ v : tuple_of ?tv |- _ ] => unfold tuple_of in v; unfold tv in v; simpl in v; unfold val; simpl SessionPrelude.value_of end;
+  lazymatch goal with [ v : tuple_of ?tv |- _ ] => unfold tuple_of in v; unfold tv in v; simpl in v; unfold val; simpl end;
   repeat constructor; auto.
 
 #[local] Tactic Notation "tac_IntoVal" integer( n ) :=
   intros;
   lazymatch goal with [ v : tuple_of ?tv |- _ ] => unfold tuple_of in v; unfold tv in v; simpl in v; simpl SessionPrelude.value_of; do n destruct v as [v ?]; simpl end;
   repeat lazymatch goal with [ t : Slice.t |- _ ] => destruct t end; auto.
+
+Definition BOUND (a: Z) (n: nat) : Prop :=
+  a >= 1 /\ Z.of_nat n <= 2 ^ 64 - a.
 
 #[universes(template)]
 Class has_value_boundary (t: Type) : Type :=
@@ -22,11 +29,29 @@ Instance u64_has_value_boundary : has_value_boundary u64 :=
 
 #[global]
 Instance nat_has_value_boundary : has_value_boundary nat :=
-  fun a: Z => fun n: nat => a >= 1 /\ Z.of_nat n <= 2 ^ 64 - a.
-  
+  BOUND.
+
+Lemma BOUND_dec a n
+  : {BOUND a n} + {~ BOUND a n}.
+Proof.
+  unfold BOUND;
+  pose proof (Z.ge_dec a 1) as [YES_ge | NO_ge];
+  pose proof (Z.le_dec (Z.of_nat n) (2 ^ 64 - a)) as [YES_le | NO_le];
+  first [now left; split | right; word].
+Qed.
+
+Lemma maybe_u64 (a: Z) (n: nat)
+  : { RET : option u64 | match RET with Some v => value_bound a n /\ uint.nat v = n | None => ~ value_bound a n end }.
+Proof.
+  pose proof (BOUND_dec a n) as [YES | NO].
+  - red in YES; exists (Some (W64 n)); split; trivial; word.
+  - exists None; trivial.
+Qed.
+
 #[global]
 Instance list_has_value_boundary {t: Type} (t_has_value_boundary: has_value_boundary t) : has_value_boundary (list t) :=
-  fun a: Z => Forall ( @value_bound t t_has_value_boundary a).
+  let has_value_boundary : has_value_boundary t := t_has_value_boundary in
+  fun a: Z => Forall (has_value_boundary a).
 
 Module _Data.
 
@@ -90,36 +115,52 @@ Module Operation.
     - refine (_). refine (Data _). exact F_A.
   Defined.
 
-  Definition size_of {u64: Type} (object: t u64) : nat :=
+  #[global, program]
+  Instance IntoVal : IntoVal (tuple_of tv) :=
+    { to_val := val
+    ; from_val := from_val
+    ; IntoVal_def := (IntoVal_def Slice.t, IntoVal_def _Data.t)
+    }.
+  Next Obligation.
+    tac_IntoVal 1.
+  Defined.
+
+  Section ADD_ON.
+
+  Context {u64: Type}.
+
+  Section HASKELLISH_INSTANCES.
+
+  Definition getVersionVector (op: Operation.t u64) : list u64 :=
+    op.(VersionVector).
+
+  Context {u64_well_formed: u64 -> Prop}.
+
+  Definition well_formed (n: nat) (op: Operation.t u64) : Prop :=
+    Forall u64_well_formed op.(VersionVector) /\ length op.(VersionVector) = n.
+
+  Context {u64_hsEq: SessionPrelude.hsEq u64 (well_formed := u64_well_formed)}.
+
+  #[global]
+  Instance hsEq_Operation (n: nat) : SessionPrelude.hsEq (Operation.t u64) (well_formed := well_formed n) :=
+    SessionPrelude.hsEq_preimage getVersionVector.
+
+  Context {u64_hsOrd: SessionPrelude.hsOrd u64 (well_formed := u64_well_formed)}.
+
+  #[global]
+  Instance hsOrd_Operation (n: nat) : SessionPrelude.hsOrd (Operation.t u64) (well_formed := well_formed n) :=
+    SessionPrelude.hsOrd_preimage getVersionVector.
+
+  End HASKELLISH_INSTANCES.
+
+  Definition size_of (object: t u64) : nat :=
     length object.(VersionVector).
+
+  Context `(has_value_boundary u64).
 
   #[global]
   Instance value_bound : has_value_boundary (t u64) :=
     fun a: Z => fun object: t u64 => value_bound a object.(VersionVector).
-
-  Section ADD_ON.
-
-    Context {u64: Type}.
-
-    Definition getVersionVector (op: Operation.t u64) : list u64 :=
-      op.(VersionVector).
-
-    Context {u64_well_formed: u64 -> Prop}.
-
-    Definition well_formed (n: nat) (op: Operation.t u64) : Prop :=
-      Forall u64_well_formed op.(VersionVector) /\ length op.(VersionVector) = n.
-
-    Context {u64_hsEq: SessionPrelude.hsEq u64 (well_formed := u64_well_formed)}.
-
-    #[global]
-    Instance hsEq_Operation (n: nat) : SessionPrelude.hsEq (Operation.t u64) (well_formed := well_formed n) :=
-      SessionPrelude.hsEq_preimage getVersionVector.
-
-    Context {u64_hsOrd: SessionPrelude.hsOrd u64 (well_formed := u64_well_formed)}.
-
-    #[global]
-    Instance hsOrd_Operation (n: nat) : SessionPrelude.hsOrd (Operation.t u64) (well_formed := well_formed n) :=
-      SessionPrelude.hsOrd_preimage getVersionVector.
 
   End ADD_ON.
 
@@ -196,13 +237,31 @@ Module Message.
     - refine (A_to_B _). refine (S2C_Client_Number _). exact F_A.
   Defined.
 
+  #[global, program]
+  Instance IntoVal : IntoVal (tuple_of tv) :=
+    { to_val := val
+    ; from_val := from_val
+    ; IntoVal_def := (W64 0, W64 0, W64 0, W64 0, IntoVal_def _Data.t, IntoVal_def Slice.t, W64 0, W64 0, IntoVal_def Slice.t, W64 0, W64 0, W64 0, W64 0, W64 0, IntoVal_def _Data.t, IntoVal_def Slice.t, W64 0, W64 0);
+    }.
+  Next Obligation.
+    tac_IntoVal 17.
+  Defined.
+
+  Section ADD_ON.
+
+  Context {u64: Type}.
+
   Definition size_of (object: t u64) : nat * nat :=
     (length object.(C2S_Client_VersionVector), length object.(S2C_Client_VersionVector)).
 
+  Context `(has_value_boundary u64).
+
   Variant _value_bound {a: Z} (object: t u64) : Prop :=
     | _value_bound_intro
+      (MessageType_bound: value_bound 1 object.(MessageType))
       (C2S_Client_Id_bound: value_bound a object.(C2S_Client_Id))
       (C2S_Server_Id_bound: value_bound a object.(C2S_Server_Id))
+      (C2S_Client_OperationType_bound: value_bound 1 object.(C2S_Client_OperationType))
       (C2S_Client_VersionVector: value_bound a object.(C2S_Client_VersionVector))
       (S2S_Gossip_Sending_ServerId_bound: value_bound a object.(S2S_Gossip_Sending_ServerId))
       (S2S_Gossip_Receiving_ServerId_bound: value_bound a object.(S2S_Gossip_Receiving_ServerId))
@@ -211,6 +270,7 @@ Module Message.
       (S2S_Acknowledge_Gossip_Sending_ServerId_bound: value_bound a object.(S2S_Acknowledge_Gossip_Sending_ServerId))
       (S2S_Acknowledge_Gossip_Receiving_ServerId_bound: value_bound a object.(S2S_Acknowledge_Gossip_Receiving_ServerId))
       (S2S_Acknowledge_Gossip_Index_bound: value_bound a object.(S2S_Acknowledge_Gossip_Index))
+      (S2C_Client_OperationType_bound: value_bound 1 object.(S2C_Client_OperationType))
       (S2C_Client_VersionVector_bound: value_bound a object.(S2C_Client_VersionVector))
       (S2C_Server_Id_bound: value_bound a object.(S2C_Server_Id))
       (S2C_Client_Number: value_bound a object.(S2C_Client_Number))
@@ -219,6 +279,8 @@ Module Message.
   #[global]
   Instance has_value_boundary : has_value_boundary (t u64) :=
     @_value_bound.
+
+  End ADD_ON.
 
 End Message.
 
@@ -269,8 +331,24 @@ Module Server.
     - refine (fmap A_to_B _). refine (GossipAcknowledgements _). exact F_A.
   Qed.
 
+  #[global, program]
+  Instance IntoVal : IntoVal (tuple_of tv) :=
+    { to_val := val
+    ; from_val := from_val
+    ; IntoVal_def := (W64 0, W64 0, IntoVal_def Slice.t, IntoVal_def Slice.t, IntoVal_def Slice.t, IntoVal_def Slice.t, IntoVal_def Slice.t, IntoVal_def Slice.t)
+    }.
+  Next Obligation.
+    tac_IntoVal 7.
+  Defined.
+
+  Section ADD_ON.
+
+  Context {u64: Type}.
+
   Definition size_of (object: t u64) : nat * nat * nat * nat * nat :=
     (length object.(VectorClock), length object.(OperationsPerformed), length object.(MyOperations), length object.(PendingOperations), length object.(GossipAcknowledgements)).
+
+  Context `(has_value_boundary u64).
 
   Variant _value_bound {a: Z} (object: t u64) : Prop :=
     | _value_bound_intro
@@ -287,6 +365,8 @@ Module Server.
   #[global]
   Instance has_value_boundary : has_value_boundary (t u64) :=
     @_value_bound.
+
+  End ADD_ON.
 
 End Server.
 
@@ -331,20 +411,39 @@ Module Client.
     - refine (A_to_B _). refine (SessionSemantic _). exact F_A.
   Defined.
 
+  #[global, program]
+  Instance IntoVal : IntoVal (tuple_of tv) :=
+    { to_val := val
+    ; from_val := from_val
+    ; IntoVal_def := (W64 0, W64 0, IntoVal_def Slice.t, IntoVal_def Slice.t, W64 0);
+    }.
+  Next Obligation.
+    tac_IntoVal 4.
+  Defined.
+
+  Section ADD_ON.
+
+  Context {u64: Type}.
+
   Definition size_of (object: t u64) : nat * nat :=
     (length object.(WriteVersionVector), length object.(ReadVersionVector)).
 
-  Variant _value_bound {a: Z} (object: t u64) : Prop :=
+  Context `(has_value_boundary u64).
+
+  Variant _value_bound {a: Z} (object: t nat) : Prop :=
     | _value_bound_intro
       (Id_bound: value_bound a object.(Id))
       (NumberOfServers_bound: value_bound a object.(NumberOfServers))
       (WriteVersionVector_bound: value_bound a object.(WriteVersionVector))
       (ReadVersionVector_bound: value_bound a object.(ReadVersionVector))
+      (SessionSemantic_bound: value_bound 1 object.(SessionSemantic))
       : _value_bound object.
 
   #[global]
-  Instance has_value_boundary : has_value_boundary (t u64) :=
+  Instance has_value_boundary : has_value_boundary (t nat) :=
     @_value_bound.
+
+  End ADD_ON.
 
 End Client.
 
@@ -360,20 +459,6 @@ Module ServerSide.
 
   #[global] Hint Resolve Operation_val_t : typeclasses_hints.
 
-  #[global]
-  Instance Operation_IntoVal
-    : IntoVal (tuple_of Operation.tv).
-  Proof.
-    refine (
-      {|
-        to_val := Operation.val;
-        from_val := Operation.from_val;
-        IntoVal_def := (IntoVal_def Slice.t, IntoVal_def _Data.t);
-      |}
-    ).
-    tac_IntoVal 1.
-  Defined.
-
   Theorem Message_val_t v
     : val_ty (Message.val v) (struct.t SessionServer.Message).
   Proof.
@@ -381,20 +466,6 @@ Module ServerSide.
   Qed.
 
   #[global] Hint Resolve Message_val_t : typeclasses_hints.
-
-  #[global]
-  Instance Message_IntoVal
-    : IntoVal (tuple_of Message.tv).
-  Proof.
-    refine (
-      {|
-        to_val := Message.val;
-        from_val := Message.from_val;
-        IntoVal_def := (W64 0, W64 0, W64 0, W64 0, IntoVal_def _Data.t, IntoVal_def Slice.t, W64 0, W64 0, IntoVal_def Slice.t, W64 0, W64 0, W64 0, W64 0, W64 0, IntoVal_def _Data.t, IntoVal_def Slice.t, W64 0, W64 0);
-      |}
-    ).
-    tac_IntoVal 17.
-  Defined.
 
   Theorem Server_val_t v
     : val_ty (Server.val v) (struct.t SessionServer.Server).
@@ -404,33 +475,21 @@ Module ServerSide.
 
   #[global] Hint Resolve Server_val_t : typeclasses_hints.
 
-  #[global]
-  Instance Server_IntoVal
-    : IntoVal (tuple_of Server.tv).
-  Proof.
-    refine (
-      {|
-        to_val := Server.val;
-        from_val := Server.from_val;
-        IntoVal_def := (W64 0, W64 0, IntoVal_def Slice.t, IntoVal_def Slice.t, IntoVal_def Slice.t, IntoVal_def Slice.t, IntoVal_def Slice.t, IntoVal_def Slice.t);
-      |}
-    ).
-    tac_IntoVal 7.
-  Defined.
-
   Section heap.
 
     Context `{hG: !heapGS Σ}.
 
-    Definition is_good_operation (v: tuple_of Operation.tv) (object: Operation.t u64) (n: nat) : iProp Σ :=
+    Definition isOperation (v: tuple_of Operation.tv) (op: Operation.t nat) (n: nat) : iProp Σ :=
+      ∃ object, ⌜Operation.FMap u64 nat (fun u : u64 => uint.nat u) object = op⌝ ∗
       own_slice_small v!(0) uint64T DfracDiscarded object.(Operation.VersionVector) ∗
       ⌜v!(1) = object.(Operation.Data)⌝ ∗
-      ⌜Operation.size_of object = n⌝.
+      ⌜Operation.size_of op = n⌝.
 
-    Definition is_good_slice_of_operations (s: Slice.t) (objects: list (Operation.t u64)) (n: nat) : iProp Σ :=
-      ∃ vs, own_slice s (struct.t Operation) (DfracOwn 1) vs ∗ [∗ list] v;o ∈ vs;objects, is_good_operation v o n.
+    Definition isOperationSlice (s: Slice.t) (ops: list (Operation.t nat)) (n: nat) : iProp Σ :=
+      ∃ vs, own_slice s (struct.t Operation) (DfracOwn 1) vs ∗ [∗ list] v;op ∈ vs;ops, isOperation v op n.
 
-    Definition is_good_message (v: tuple_of Message.tv) (object: Message.t u64) (n: nat) (len_c2s: nat) (len_s2c: nat) : iProp Σ :=
+    Definition isMessage (v: tuple_of Message.tv) (msg: Message.t nat) (n: nat) (len_c2s: nat) (len_s2c: nat) : iProp Σ :=
+      ∃ object, ⌜Message.FMap u64 nat (fun u : u64 => uint.nat u) object = msg⌝ ∗
       ⌜v!(0) = object.(Message.MessageType)⌝ ∗
       ⌜v!(1) = object.(Message.C2S_Client_Id)⌝ ∗
       ⌜v!(2) = object.(Message.C2S_Server_Id)⌝ ∗
@@ -440,7 +499,7 @@ Module ServerSide.
       ⌜len_c2s = length object.(Message.C2S_Client_VersionVector)⌝ ∗
       ⌜v!(6) = object.(Message.S2S_Gossip_Sending_ServerId)⌝ ∗
       ⌜v!(7) = object.(Message.S2S_Gossip_Receiving_ServerId)⌝ ∗
-      is_good_slice_of_operations v!(8) object.(Message.S2S_Gossip_Operations) n ∗
+      isOperationSlice v!(8) msg.(Message.S2S_Gossip_Operations) n ∗
       ⌜v!(9) = object.(Message.S2S_Gossip_Index)⌝ ∗
       ⌜v!(10) = object.(Message.S2S_Acknowledge_Gossip_Sending_ServerId)⌝ ∗
       ⌜v!(11) = object.(Message.S2S_Acknowledge_Gossip_Receiving_ServerId)⌝ ∗
@@ -450,29 +509,282 @@ Module ServerSide.
       own_slice_small v!(15) uint64T (DfracOwn 1) object.(Message.S2C_Client_VersionVector) ∗
       ⌜v!(16) = object.(Message.S2C_Server_Id)⌝ ∗
       ⌜v!(17) = object.(Message.S2C_Client_Number)⌝ ∗
-      ⌜Message.size_of object = (len_c2s, len_s2c)⌝.
+      ⌜Message.size_of msg = (len_c2s, len_s2c)⌝.
 
-    Definition is_good_slice_of_messages (s: Slice.t) (objects: list (Message.t u64)) (n: nat) (len_c2s: nat) : iProp Σ :=
-      ∃ vs, own_slice s (struct.t Message) (DfracOwn 1) vs ∗ [∗ list] v;o ∈ vs;objects, ∃ len_s2c : nat, is_good_message v o n len_c2s len_s2c.
+    Definition isMessageSlice (s: Slice.t) (msgs: list (Message.t nat)) (n: nat) (len_c2s: nat) : iProp Σ :=
+      ∃ vs, own_slice s (struct.t Message) (DfracOwn 1) vs ∗ [∗ list] v;msg ∈ vs;msgs, ∃ len_s2c : nat, isMessage v msg n len_c2s len_s2c.
 
-    Definition is_good_server' {OWN_UnsatisfiedRequests: bool} (v: tuple_of Server.tv) (object: Server.t u64) (n: nat) (len_vc: nat) (len_op: nat) (len_mo: nat) (len_po: nat) (len_ga: nat) : iProp Σ :=
+    Definition isServer' {OWN_UnsatisfiedRequests: bool} (v: tuple_of Server.tv) (server: Server.t nat) (n: nat) (len_vc: nat) (len_op: nat) (len_mo: nat) (len_po: nat) (len_ga: nat) : iProp Σ :=
+      ∃ object, ⌜Server.FMap u64 nat (fun u : u64 => uint.nat u) object = server⌝ ∗
       ⌜v!(0) = object.(Server.Id)⌝ ∗
       ⌜v!(1) = object.(Server.NumberOfServers)⌝ ∗
-      (if OWN_UnsatisfiedRequests then is_good_slice_of_messages v!(2) object.(Server.UnsatisfiedRequests) n len_vc else emp)%I ∗
+      (if OWN_UnsatisfiedRequests then isMessageSlice v!(2) server.(Server.UnsatisfiedRequests) n len_vc else emp)%I ∗
       own_slice_small v!(3) uint64T (DfracOwn 1) object.(Server.VectorClock) ∗
-      is_good_slice_of_operations v!(4) object.(Server.OperationsPerformed) len_op ∗
-      is_good_slice_of_operations v!(5) object.(Server.MyOperations) len_mo ∗
-      is_good_slice_of_operations v!(6) object.(Server.PendingOperations) len_po ∗
+      isOperationSlice v!(4) server.(Server.OperationsPerformed) len_op ∗
+      isOperationSlice v!(5) server.(Server.MyOperations) len_mo ∗
+      isOperationSlice v!(6) server.(Server.PendingOperations) len_po ∗
       own_slice_small v!(7) uint64T (DfracOwn 1) object.(Server.GossipAcknowledgements) ∗
-      ⌜Server.size_of object = (len_vc, len_op, len_mo, len_po, len_ga)⌝.
+      ⌜Server.size_of server = (len_vc, len_op, len_mo, len_po, len_ga)⌝.
 
   End heap.
 
-  Notation is_good_server := (is_good_server' (OWN_UnsatisfiedRequests := true)).
+  Notation isServer := (isServer' (OWN_UnsatisfiedRequests := true)).
 
   Section Coq_nat.
 
-    (* TODO *)
+  #[local] Open Scope nat_scope.
+
+  Fixpoint coq_compareVersionVector (v1: list nat) (v2: list nat) : bool :=
+    match v1 with
+    | [] => true
+    | h1 :: t1 =>
+      match v2 with
+      | [] => true
+      | h2 :: t2 => (h2 <=? h1)%nat && (coq_compareVersionVector t1 t2)
+      end
+    end.
+
+  Fixpoint coq_lexicographicCompare (v1: list nat) (v2: list nat) : bool :=
+    match v1 with
+    | [] => false
+    | h1 :: t1 =>
+      match v2 with
+      | [] => false
+      | h2 :: t2 => if (h1 =? h2)%nat then coq_lexicographicCompare t1 t2 else (h2 <? h1)%nat
+      end
+    end.
+
+  Definition coq_maxTwoInts (x: nat) (y: nat) : nat :=
+    Nat.max x y.
+
+  Fixpoint coq_maxTS (v1: list nat) (v2: list nat) : list nat :=
+    match v1 with
+    | [] => []
+    | hd1 :: tl1 =>
+      match v2 with
+      | [] => []
+      | hd2 :: tl2 => coq_maxTwoInts hd1 hd2 :: coq_maxTS tl1 tl2
+      end
+    end.
+
+  Definition coq_oneOffVersionVector (v1: list nat) (v2: list nat) : bool :=
+    let loop_step (acc: bool * bool) (elem: nat * nat) : bool * bool :=
+      let (e1, e2) := elem in
+      let (output, canApply) := acc in
+      if canApply && (e1 + 1 =? e2)%nat then
+        (output, false)
+      else if (e2 <=? e1)%nat then
+        (output, canApply)
+      else 
+        (false, canApply)
+    in
+    let (output, canApply) := fold_left loop_step (zip v1 v2) (true, true) in
+    output && negb canApply.
+
+  Fixpoint coq_equalSlices (s1: list nat) (s2: list nat) : bool :=
+    match s1 with
+    | [] => true
+    | h1 :: t1 =>
+      match s2 with
+      | [] => true
+      | h2 :: t2 => (h1 =? h2)%nat && coq_equalSlices t1 t2
+      end
+    end.
+
+  Variant binarySearch_spec (needle: Operation.t nat) (l: list (Operation.t nat)) (n: nat) (RESULT: nat) : Prop :=
+    | binarySearch_spec_intro (prefix: list (list nat)) (suffix: list (list nat))
+      (LENGTH: RESULT = length prefix)
+      (VECTOR: map Operation.getVersionVector l = if forallb (fun x => negb (coq_equalSlices x.(Operation.VersionVector) needle.(Operation.VersionVector))) l then prefix ++ suffix else prefix ++ [Operation.getVersionVector needle] ++ suffix)
+      (PREFIX: ∀ op, In op prefix -> coq_lexicographicCompare needle.(Operation.VersionVector) op = true)
+      (SUFFIX: ∀ op, In op suffix -> coq_lexicographicCompare op needle.(Operation.VersionVector) = true)
+      : binarySearch_spec needle l n RESULT.
+
+  Fixpoint coq_sortedInsert (l: list (Operation.t nat)) (i: Operation.t nat) : list (Operation.t nat) :=
+    match l with
+    | [] => [i]
+    | h :: t =>
+      if coq_lexicographicCompare h.(Operation.VersionVector) i.(Operation.VersionVector) then
+        i :: h :: t
+      else if coq_equalSlices h.(Operation.VersionVector) i.(Operation.VersionVector) then
+        h :: t
+      else
+        h :: coq_sortedInsert t i
+    end.
+
+  Definition coq_deleteAtIndexOperation (ops: list (Operation.t nat)) (index: nat) : list (Operation.t nat) :=
+    take index ops ++ drop (index + 1)%nat ops.
+
+  Definition coq_deleteAtIndexMessage (msgs: list (Message.t nat)) (index: nat) : list (Message.t nat) :=
+    take index msgs ++ drop (index + 1)%nat msgs.
+
+  Definition coq_getDataFromOperationLog (l: list (Operation.t nat)) : _Data.t :=
+    match last l with
+    | Some v => v.(Operation.Data)
+    | None => IntoVal_def _Data.t
+    end.
+
+  Definition coq_receiveGossip (server: Server.t nat) (request: Message.t nat) : Server.t nat :=
+    if (length request.(Message.S2S_Gossip_Operations) =? 0)%nat then
+      server
+    else
+      let first_loop_output : Server.t nat :=
+        let focus := request.(Message.S2S_Gossip_Operations) in
+        let loop_step (acc: Server.t nat) (elem: Operation.t nat) : Server.t nat :=
+          let server := acc in
+          if coq_oneOffVersionVector server.(Server.VectorClock) elem.(Operation.VersionVector) then
+            {|
+              Server.Id := server.(Server.Id);
+              Server.NumberOfServers := server.(Server.NumberOfServers);
+              Server.UnsatisfiedRequests := server.(Server.UnsatisfiedRequests);
+              Server.VectorClock := coq_maxTS server.(Server.VectorClock) elem.(Operation.VersionVector);
+              Server.OperationsPerformed := coq_sortedInsert server.(Server.OperationsPerformed) elem;
+              Server.MyOperations := server.(Server.MyOperations);
+              Server.PendingOperations := server.(Server.PendingOperations);
+              Server.GossipAcknowledgements := server.(Server.GossipAcknowledgements);
+            |}
+          else if negb (coq_compareVersionVector server.(Server.VectorClock) elem.(Operation.VersionVector)) then
+            {|
+              Server.Id := server.(Server.Id);
+              Server.NumberOfServers := server.(Server.NumberOfServers);
+              Server.UnsatisfiedRequests := server.(Server.UnsatisfiedRequests);
+              Server.VectorClock := server.(Server.VectorClock);
+              Server.OperationsPerformed := server.(Server.OperationsPerformed);
+              Server.MyOperations := server.(Server.MyOperations);
+              Server.PendingOperations := coq_sortedInsert server.(Server.PendingOperations) elem;
+              Server.GossipAcknowledgements := server.(Server.GossipAcknowledgements);
+            |}
+          else
+            server
+        in
+        fold_left loop_step focus server
+      in
+      let server := first_loop_output in
+      let second_loop_output : Server.t nat * nat * list nat :=
+        let focus := server.(Server.PendingOperations) in
+        let loop_step (acc: Server.t nat * nat * list nat) (elem: Operation.t nat) : Server.t nat * nat * list nat :=
+          let '(server, i, seen) := acc in
+            if coq_oneOffVersionVector server.(Server.VectorClock) elem.(Operation.VersionVector) then
+              (Server.mk _ server.(Server.Id) server.(Server.NumberOfServers) server.(Server.UnsatisfiedRequests) (coq_maxTS server.(Server.VectorClock) elem.(Operation.VersionVector)) (coq_sortedInsert server.(Server.OperationsPerformed) elem) server.(Server.MyOperations) server.(Server.PendingOperations) server.(Server.GossipAcknowledgements), (i + 1)%nat, seen ++ [i])
+            else
+              (server, (i + 1)%nat, seen)
+        in
+        fold_left loop_step focus (server, 0%nat, [])
+      in
+      let '(server, _, seen) := second_loop_output in
+      let third_loop_output : nat * nat * list (Operation.t nat) :=
+        let focus := server.(Server.PendingOperations) in
+        let loop_step (acc: nat * nat * list (Operation.t nat)) (elem: Operation.t nat) : nat * nat * list (Operation.t nat) :=
+          let '(i, j, output) := acc in
+          match seen !! j with
+          | Some i' => if (i =? i')%nat then ((i + 1)%nat, (j + 1)%nat, output) else ((i + 1)%nat, j, output ++ [elem])
+          | None => ((i + 1)%nat, j, output ++ [elem])
+          end
+        in
+        fold_left loop_step focus (0%nat, 0%nat, [])
+      in
+      let '(_, _, output) := third_loop_output in
+      {|
+        Server.Id := server.(Server.Id);
+        Server.NumberOfServers := server.(Server.NumberOfServers);
+        Server.UnsatisfiedRequests := server.(Server.UnsatisfiedRequests);
+        Server.VectorClock := server.(Server.VectorClock);
+        Server.OperationsPerformed := server.(Server.OperationsPerformed);
+        Server.MyOperations := server.(Server.MyOperations);
+        Server.PendingOperations := output;
+        Server.GossipAcknowledgements := server.(Server.GossipAcknowledgements);
+      |}.
+
+  Definition coq_acknowledgeGossip (s: Server.t nat) (r: Message.t nat) : Server.t nat :=
+    let i := r.(Message.S2S_Acknowledge_Gossip_Sending_ServerId) in
+    let l := s.(Server.GossipAcknowledgements) in
+    if (i <? length l)%nat then
+      let prevGossipAcknowledgementsValue : nat :=
+        match s.(Server.GossipAcknowledgements) !! i with
+        | Some x => x
+        | None => 0%nat
+        end
+      in
+      let newGossipAcknowledgements := coq_maxTwoInts prevGossipAcknowledgementsValue r.(Message.S2S_Acknowledge_Gossip_Index) in
+      let gossipAcknowledgements := <[i := newGossipAcknowledgements]> l in
+      Server.mk _ s.(Server.Id) s.(Server.NumberOfServers) s.(Server.UnsatisfiedRequests) s.(Server.VectorClock) s.(Server.OperationsPerformed) s.(Server.MyOperations) s.(Server.PendingOperations) gossipAcknowledgements
+    else
+      s.
+
+  Definition coq_getGossipOperations (s: Server.t nat) (serverId: nat) : list (Operation.t nat) :=
+    match s.(Server.GossipAcknowledgements) !! serverId with
+    | Some v => drop v s.(Server.MyOperations)
+    | None => []
+    end.
+
+  Definition coq_processClientRequest (s: Server.t nat) (r: Message.t nat) : bool * Server.t nat * Message.t nat :=
+    if coq_compareVersionVector s.(Server.VectorClock) r.(Message.C2S_Client_VersionVector) then
+      if (r.(Message.C2S_Client_OperationType) =? 0)%nat then
+        let S2C_Client_Data := coq_getDataFromOperationLog s.(Server.OperationsPerformed) in
+        let S2C_Client_VersionVector := s.(Server.VectorClock) in
+        let S2C_Client_Number := r.(Message.C2S_Client_Id) in
+        let S2C_Server_Id := s.(Server.Id) in
+        (true, s, Message.mk nat 4 0 0 0 (IntoVal_def _Data.t) [] 0 0 [] 0 0 0 0 0 S2C_Client_Data S2C_Client_VersionVector S2C_Server_Id S2C_Client_Number)
+      else
+        let v := match s.(Server.VectorClock) !! s.(Server.Id) with Some v => v | None => 0 end in
+        let VectorClock := <[s.(Server.Id) := (v + 1)%nat]> s.(Server.VectorClock) in
+        let OperationsPerformed := coq_sortedInsert s.(Server.OperationsPerformed) (Operation.mk nat VectorClock r.(Message.C2S_Client_Data)) in
+        let MyOperations := coq_sortedInsert s.(Server.MyOperations) (Operation.mk nat VectorClock r.(Message.C2S_Client_Data)) in
+        let S2C_Client_OperationType := 1 in
+        let S2C_Client_Data := IntoVal_def _Data.t in
+        let S2C_Client_VersionVector := VectorClock in
+        let S2C_Client_Number := r.(Message.C2S_Client_Id) in
+        let S2C_Server_Id := s.(Server.Id) in
+        (true, Server.mk nat s.(Server.Id) s.(Server.NumberOfServers) s.(Server.UnsatisfiedRequests) VectorClock OperationsPerformed MyOperations s.(Server.PendingOperations) s.(Server.GossipAcknowledgements), Message.mk nat 4 0 0 0 (W64 0) [] 0 0 [] 0 0 0 0 1 S2C_Client_Data S2C_Client_VersionVector S2C_Server_Id S2C_Client_Number)
+    else
+      (false, s, Message.mk nat 0 0 0 0 (IntoVal_def _Data.t) [] 0 0 [] 0 0 0 0 0 (IntoVal_def _Data.t) [] 0 0).
+
+  Definition coq_processRequest (server: Server.t nat) (request: Message.t nat) : Server.t nat * list (Message.t nat) :=
+    match request.(Message.MessageType) with
+    | 0%nat =>
+      let '(succeeded, server, reply) := coq_processClientRequest server request in
+      if succeeded then
+        (server, [reply])
+      else
+        let UnsatisfiedRequests := server.(Server.UnsatisfiedRequests) ++ [request] in 
+        let server := Server.mk nat server.(Server.Id) server.(Server.NumberOfServers) UnsatisfiedRequests server.(Server.VectorClock) server.(Server.OperationsPerformed) server.(Server.MyOperations) server.(Server.PendingOperations) server.(Server.GossipAcknowledgements) in
+        (server, [])
+    | 1%nat =>
+      let server := coq_receiveGossip server request in
+      let focus := server.(Server.UnsatisfiedRequests) in
+      let loop_init : nat * Server.t nat * list (Message.t nat) :=
+        (0%nat, server, [])
+      in
+      let loop_step (acc: nat * Server.t nat * list (Message.t nat)) (element: Message.t nat) : nat * Server.t nat * list (Message.t nat) :=
+        let '(i, s, outGoingRequests) := acc in
+        let '(succeeded, s, reply) := coq_processClientRequest s element in
+        if succeeded then
+          let UnsatisfiedRequests := coq_deleteAtIndexMessage s.(Server.UnsatisfiedRequests) i in
+          (i, Server.mk nat s.(Server.Id) s.(Server.NumberOfServers) UnsatisfiedRequests s.(Server.VectorClock) s.(Server.OperationsPerformed) s.(Server.MyOperations) s.(Server.PendingOperations) s.(Server.GossipAcknowledgements), outGoingRequests ++ [reply])
+        else
+          ((i + 1)%nat, s, outGoingRequests)
+      in
+      let '(_, server, outGoingRequests) := fold_left loop_step focus loop_init in
+      (server, outGoingRequests)
+    | 2%nat => (coq_acknowledgeGossip server request, [])
+    | 3%nat =>
+      let loop_step (acc: Server.t nat * list (Message.t nat)) (index: nat) : Server.t nat * list (Message.t nat) :=
+        let '(server, outGoingRequests) := acc in
+        let operations := coq_getGossipOperations server index in
+        if negb (index =? server.(Server.Id))%nat && negb (length operations =? 0)%nat then
+          let GossipAcknowledgements := <[index := length server.(Server.MyOperations)]> server.(Server.GossipAcknowledgements) in
+          let S2S_Gossip_Sending_ServerId := server.(Server.Id) in
+          let S2S_Gossip_Receiving_ServerId := index in
+          let S2S_Gossip_Operations := operations in
+          let S2S_Gossip_Index := length (server.(Server.MyOperations)) in
+          let message := Message.mk nat 1 0 0 0 (IntoVal_def _Data.t) [] S2S_Gossip_Sending_ServerId S2S_Gossip_Receiving_ServerId S2S_Gossip_Operations S2S_Gossip_Index 0 0 0 0 (IntoVal_def _Data.t) [] 0 0 in
+          (Server.mk nat server.(Server.Id) server.(Server.NumberOfServers) server.(Server.UnsatisfiedRequests) server.(Server.VectorClock) server.(Server.OperationsPerformed) server.(Server.MyOperations) server.(Server.PendingOperations) GossipAcknowledgements, outGoingRequests ++ [message])
+        else
+          (server, outGoingRequests)
+      in
+      let focus := seq 0%nat server.(Server.NumberOfServers) in
+      fold_left loop_step focus (server, [])
+    | _ => (server, [])
+    end.
 
   End Coq_nat.
 
@@ -490,13 +802,6 @@ Module ClientSide.
 
   #[global] Hint Resolve Operation_val_t : typeclasses_hints.
 
-  #[global]
-  Instance Operation_IntoVal
-    : IntoVal (tuple_of Operation.tv).
-  Proof.
-    exact (ServerSide.Operation_IntoVal).
-  Defined.
-
   Theorem Message_val_t v
     : val_ty (Message.val v) (struct.t SessionClient.Message).
   Proof.
@@ -504,13 +809,6 @@ Module ClientSide.
   Defined.
 
   #[global] Hint Resolve Message_val_t : typeclasses_hints.
-
-  #[global]
-  Instance Message_IntoVal
-    : IntoVal (tuple_of Message.tv).
-  Proof.
-    exact (ServerSide.Message_IntoVal).
-  Defined.
 
   Theorem Client_val_t v
     : val_ty (Client.val v) (struct.t SessionClient.Client).
@@ -520,47 +818,69 @@ Module ClientSide.
 
   #[global] Hint Resolve Client_val_t : typeclasses_hints.
 
-  #[global]
-  Instance Client_IntoVal
-    : IntoVal (tuple_of Client.tv).
-  Proof.
-    refine (
-      {|
-        to_val := Client.val;
-        from_val := Client.from_val;
-        IntoVal_def := (W64 0, W64 0, IntoVal_def Slice.t, IntoVal_def Slice.t, W64 0);
-      |}
-    ).
-    tac_IntoVal 4.
-  Defined.
+  Notation isOperation := ServerSide.isOperation.
 
-  Notation is_good_operation := ServerSide.is_good_operation.
+  Notation isOperationSlice := ServerSide.isOperationSlice.
 
-  Notation is_good_slice_of_operations := ServerSide.is_good_slice_of_operations.
+  Notation isMessage := ServerSide.isMessage.
 
-  Notation is_good_message := ServerSide.is_good_message.
-
-  Notation is_good_slice_of_messages := ServerSide.is_good_slice_of_messages.
+  Notation isMessageSlice := ServerSide.isMessageSlice.
 
   Section heap.
 
-    Context `{hG: !heapGS Σ}.
+  Context `{hG: !heapGS Σ}.
 
-    Definition is_good_client (v: tuple_of Client.tv) (object: Client.t u64) (n: nat) : iProp Σ :=
-      ⌜v!(0) = object.(Client.Id)⌝ ∗
-      ⌜v!(1) = object.(Client.NumberOfServers)⌝ ∗
-      own_slice_small v!(2) uint64T (DfracOwn 1) object.(Client.WriteVersionVector) ∗
-      own_slice_small v!(3) uint64T (DfracOwn 1) object.(Client.ReadVersionVector) ∗
-      ⌜v!(4) = object.(Client.SessionSemantic)⌝ ∗
-      ⌜(Client.size_of object, uint.nat object.(Client.NumberOfServers)) = (n, n, n)⌝.
+  Definition Client_u64 (v: tuple_of Client.tv) (client: Client.t nat) (n: nat) : iProp Σ :=
+    ∃ object, ⌜Client.FMap u64 nat (fun u : u64 => uint.nat u) object = client⌝ ∗
+    ⌜v!(0) = object.(Client.Id)⌝ ∗
+    ⌜v!(1) = object.(Client.NumberOfServers)⌝ ∗
+    own_slice_small v!(2) uint64T (DfracOwn 1) object.(Client.WriteVersionVector) ∗
+    own_slice_small v!(3) uint64T (DfracOwn 1) object.(Client.ReadVersionVector) ∗
+    ⌜v!(4) = object.(Client.SessionSemantic)⌝ ∗
+    ⌜(Client.size_of client, uint.nat client.(Client.NumberOfServers)) = (n, n, n)⌝.
 
   End heap.
 
   Section Coq_nat.
 
-    Import ServerSide.
+  #[local] Open Scope nat_scope.
 
-    (* TODO *)
+  Import ServerSide.
+
+  Definition coq_read (c: Client.t nat) (serverId: nat) : Message.t nat :=
+    match c.(Client.SessionSemantic) with
+    | 0%nat => Message.mk nat 0 c.(Client.Id) serverId 0 (IntoVal_def _Data.t) (replicate c.(Client.NumberOfServers) 0) 0 0 [] 0 0 0 0 0 (IntoVal_def _Data.t) [] 0 0
+    | 1%nat => Message.mk nat 0 c.(Client.Id) serverId 0 (IntoVal_def _Data.t) (replicate c.(Client.NumberOfServers) 0) 0 0 [] 0 0 0 0 0 (IntoVal_def _Data.t) [] 0 0
+    | 2%nat => Message.mk nat 0 c.(Client.Id) serverId 0 (IntoVal_def _Data.t) (replicate c.(Client.NumberOfServers) 0) 0 0 [] 0 0 0 0 0 (IntoVal_def _Data.t) [] 0 0
+    | 3%nat => Message.mk nat 0 c.(Client.Id) serverId 0 (IntoVal_def _Data.t) c.(Client.ReadVersionVector) 0 0 [] 0 0 0 0 0 (IntoVal_def _Data.t) [] 0 0
+    | 4%nat => Message.mk nat 0 c.(Client.Id) serverId 0 (IntoVal_def _Data.t) c.(Client.WriteVersionVector) 0 0 [] 0 0 0 0 0 (IntoVal_def _Data.t) [] 0 0
+    | 5%nat => Message.mk nat 0 c.(Client.Id) serverId 0 (IntoVal_def _Data.t) (coq_maxTS c.(Client.WriteVersionVector) c.(Client.ReadVersionVector)) 0 0 [] 0 0 0 0 0 (IntoVal_def _Data.t) [] 0 0
+    | _ => Message.mk nat 0 0 0 0 (IntoVal_def _Data.t) [] 0 0 [] 0 0 0 0 0 (IntoVal_def _Data.t) [] 0 0
+    end.
+
+  Definition coq_write (c: Client.t nat) (serverId: nat) (value: _Data.t) : Message.t nat :=
+    match c.(Client.SessionSemantic) with
+    | 0%nat => Message.mk nat 0 c.(Client.Id) serverId 1 value (replicate c.(Client.NumberOfServers) 0) 0 0 [] 0 0 0 0 0 (IntoVal_def _Data.t) [] 0 0
+    | 1%nat => Message.mk nat 0 c.(Client.Id) serverId 1 value (replicate c.(Client.NumberOfServers) 0) 0 0 [] 0 0 0 0 0 (IntoVal_def _Data.t) [] 0 0
+    | 2%nat => Message.mk nat 0 c.(Client.Id) serverId 1 value (replicate c.(Client.NumberOfServers) 0) 0 0 [] 0 0 0 0 0 (IntoVal_def _Data.t) [] 0 0
+    | 3%nat => Message.mk nat 0 c.(Client.Id) serverId 1 value c.(Client.ReadVersionVector) 0 0 [] 0 0 0 0 0 (IntoVal_def _Data.t) [] 0 0
+    | 4%nat => Message.mk nat 0 c.(Client.Id) serverId 1 value c.(Client.WriteVersionVector) 0 0 [] 0 0 0 0 0 (IntoVal_def _Data.t) [] 0 0
+    | 5%nat => Message.mk nat 0 c.(Client.Id) serverId 1 value (coq_maxTS c.(Client.WriteVersionVector) c.(Client.ReadVersionVector)) 0 0 [] 0 0 0 0 0 (IntoVal_def _Data.t) [] 0 0
+    | _ => Message.mk nat 0 0 0 0 (IntoVal_def _Data.t) [] 0 0 [] 0 0 0 0 0 (IntoVal_def _Data.t) [] 0 0
+    end.
+
+  Definition coq_processRequest (c: Client.t nat) (requestType: nat) (serverId: nat) (value: _Data.t) (ackMessage: Message.t nat) : Client.t nat * Message.t nat :=
+    match requestType with
+    | 0%nat => (c, coq_read c serverId)
+    | 1%nat => (c, coq_write c serverId value)
+    | 2%nat =>
+      match ackMessage.(Message.S2C_Client_OperationType) with
+      | 0%nat => (Client.mk nat c.(Client.Id) c.(Client.NumberOfServers) c.(Client.WriteVersionVector) ackMessage.(Message.S2C_Client_VersionVector) c.(Client.SessionSemantic), Message.mk nat 0 0 0 0 (IntoVal_def _Data.t) [] 0 0 [] 0 0 0 0 0 (IntoVal_def _Data.t) [] 0 0)
+      | 1%nat => (Client.mk nat c.(Client.Id) c.(Client.NumberOfServers) ackMessage.(Message.S2C_Client_VersionVector) c.(Client.ReadVersionVector) c.(Client.SessionSemantic), Message.mk nat 0 0 0 0 (IntoVal_def _Data.t) [] 0 0 [] 0 0 0 0 0 (IntoVal_def _Data.t) [] 0 0)
+      | _ => (c, Message.mk nat 0 0 0 0 (IntoVal_def _Data.t) [] 0 0 [] 0 0 0 0 0 (IntoVal_def _Data.t) [] 0 0)
+      end
+    | _ => (c, Message.mk nat 0 0 0 0 (IntoVal_def _Data.t) [] 0 0 [] 0 0 0 0 0 (IntoVal_def _Data.t) [] 0 0)
+    end.
 
   End Coq_nat.
 
@@ -568,29 +888,29 @@ End ClientSide.
 
 Section heap.
 
-  Import ServerSide.
+Import ServerSide.
 
-  Context `{hG: !heapGS Σ}.
+Context `{hG: !heapGS Σ}.
 
-  Lemma Operation_well_formed (n: nat) v op
-    : (is_good_operation v op n)%I ⊢@{iProp Σ} (⌜Operation.well_formed (u64_well_formed := fun _ : u64 => True) n op⌝)%I.
-  Proof.
-    iIntros "H_hd". iDestruct "H_hd" as "(H3 & %H2 & %H1)"; iClear "H3".
-    iPureIntro; split; [eapply SessionPrelude.Forall_True | done].
-  Qed.
+Lemma Operation_well_formed (n: nat) v op
+  : (isOperation v op n)%I ⊢@{iProp Σ} (⌜Operation.well_formed (u64_well_formed := fun _ => True) n op⌝)%I.
+Proof.
+  iIntros "H_hd". iDestruct "H_hd" as "(%object & H_object & H3 & %H2 & %H1)"; iClear "H3".
+  iPureIntro; split; [eapply SessionPrelude.Forall_True | done].
+Qed.
 
-  Lemma Forall_Operation_well_formed (n: nat) vs ops
-    : ([∗ list] v;op ∈ vs;ops, is_good_operation v op n)%I ⊢@{iProp Σ} (⌜Forall (Operation.well_formed (u64_well_formed := fun _ : u64 => True) n) ops⌝)%I.
-  Proof.
-    revert vs; induction ops as [ | hd tl IH]; intros vs.
-    - iIntros "H_big_sepL2"; iPureIntro; eauto.
-    - iIntros "H_big_sepL2".
-      iPoseProof (big_sepL2_cons_inv_r with "H_big_sepL2") as "(%hd' & %tl' & -> & H_hd & H_tl)".
-      iAssert (⌜Operation.well_formed n hd⌝)%I as "%YES1".
-      { iApply Operation_well_formed. iExact "H_hd". }
-      iAssert (⌜Forall (Operation.well_formed n) tl⌝)%I as "%YES2".
-      { iApply IH; iExact "H_tl". }
-      iPureIntro; econstructor; trivial.
-  Qed.
+Lemma Forall_Operation_well_formed (n: nat) vs ops
+  : ([∗ list] v;op ∈ vs;ops, isOperation v op n)%I ⊢@{iProp Σ} (⌜Forall (Operation.well_formed (u64_well_formed := fun _ => True) n) ops⌝)%I.
+Proof.
+  revert vs; induction ops as [ | hd tl IH]; intros vs.
+  - iIntros "H_big_sepL2"; iPureIntro; eauto.
+  - iIntros "H_big_sepL2".
+    iPoseProof (big_sepL2_cons_inv_r with "H_big_sepL2") as "(%hd' & %tl' & -> & H_hd & H_tl)".
+    iAssert (⌜Operation.well_formed n hd⌝)%I as "%YES1".
+    { iApply Operation_well_formed. iExact "H_hd". }
+    iAssert (⌜Forall (Operation.well_formed n) tl⌝)%I as "%YES2".
+    { iApply IH; iExact "H_tl". }
+    iPureIntro; econstructor; trivial.
+Qed.
 
 End heap.
