src/program_proof/session/session_prelude.v
@@ -1,8 +1,4 @@
 From Perennial.program_proof Require Export std_proof grove_prelude.
-From Goose.session Require server client.
-
-Module SessionServer := Goose.session.server.
-Module SessionClient := Goose.session.client.
 
 Module Tac.
 
@@ -54,181 +50,181 @@ Module SessionPrelude.
 
   Section MORE_LIST_LEMMAS.
 
-    Lemma replicate_nil {A : Type}
-      : forall x : A, forall n : nat, n = 0%nat -> replicate n x = [].
-    Proof.
-      intros; subst; reflexivity.
-    Qed.
+  Lemma replicate_nil {A : Type}
+    : forall x : A, forall n : nat, n = 0%nat -> replicate n x = [].
+  Proof.
+    intros; subst; reflexivity.
+  Qed.
 
-    Lemma lookup_map {A : Type} {B : Type} (f : A -> B) (xs : list A) (i : nat)
-      : map f xs !! i = match xs !! i with Some x => Some (f x) | None => None end.
-    Proof.
-      revert i. induction xs as [ | x xs IH], i as [ | i]; simpl in *; try congruence; eauto.
-    Qed.
+  Lemma lookup_map {A : Type} {B : Type} (f : A -> B) (xs : list A) (i : nat)
+    : map f xs !! i = match xs !! i with Some x => Some (f x) | None => None end.
+  Proof.
+    revert i. induction xs as [ | x xs IH], i as [ | i]; simpl in *; try congruence; eauto.
+  Qed.
 
-    Lemma map_take {A : Type} {B : Type} (f : A -> B) (xs : list A) (n : nat)
-      : map f (take n xs) = take n (map f xs).
-    Proof.
-      revert n. induction xs as [ | x xs IH], n as [ | n]; simpl; intros; try congruence.
-    Qed.
+  Lemma map_take {A : Type} {B : Type} (f : A -> B) (xs : list A) (n : nat)
+    : map f (take n xs) = take n (map f xs).
+  Proof.
+    revert n. induction xs as [ | x xs IH], n as [ | n]; simpl; intros; try congruence.
+  Qed.
 
-    Lemma map_drop {A : Type} {B : Type} (f : A -> B) (xs : list A) (n : nat)
-      : map f (drop n xs) = drop n (map f xs).
-    Proof.
-      revert n. induction xs as [ | x xs IH], n as [ | n]; simpl; intros; try congruence.
-    Qed.
+  Lemma map_drop {A : Type} {B : Type} (f : A -> B) (xs : list A) (n : nat)
+    : map f (drop n xs) = drop n (map f xs).
+  Proof.
+    revert n. induction xs as [ | x xs IH], n as [ | n]; simpl; intros; try congruence.
+  Qed.
 
-    Context {A : Type}.
+  Context {A : Type}.
 
-    Lemma lookup_one (x1 : A) (i : nat)
-      : forall x, [x1] !! i = Some x <-> (x1 = x /\ i = 0%nat).
-    Proof.
-      intros x; split.
-      - destruct i as [ | i]; simpl in *; intros EQ; try now split. split; congruence.
-      - now intros [-> ->].
-    Qed.
+  Lemma lookup_one (x1 : A) (i : nat)
+    : forall x, [x1] !! i = Some x <-> (x1 = x /\ i = 0%nat).
+  Proof.
+    intros x; split.
+    - destruct i as [ | i]; simpl in *; intros EQ; try now split. split; congruence.
+    - now intros [-> ->].
+  Qed.
 
-    Lemma lookup_app (xs1 : list A) (xs2 : list A) (i : nat)
-      : forall x, (xs1 ++ xs2) !! i = Some x <-> (if Nat.ltb i (length xs1) then xs1 !! i = Some x else xs2 !! (i - length xs1)%nat = Some x).
-    Proof.
-      intros x. destruct (Nat.ltb _ _) as [ | ] eqn: H_OBS; [rewrite Nat.ltb_lt in H_OBS | rewrite Nat.ltb_nlt in H_OBS].
-      - rewrite lookup_app_l; try word. reflexivity.
-      - rewrite lookup_app_r; try word. reflexivity.
-    Qed.
+  Lemma lookup_app (xs1 : list A) (xs2 : list A) (i : nat)
+    : forall x, (xs1 ++ xs2) !! i = Some x <-> (if Nat.ltb i (length xs1) then xs1 !! i = Some x else xs2 !! (i - length xs1)%nat = Some x).
+  Proof.
+    intros x. destruct (Nat.ltb _ _) as [ | ] eqn: H_OBS; [rewrite Nat.ltb_lt in H_OBS | rewrite Nat.ltb_nlt in H_OBS].
+    - rewrite lookup_app_l; try word. reflexivity.
+    - rewrite lookup_app_r; try word. reflexivity.
+  Qed.
 
-    Lemma list_ext (xs : list A) (ys : list A)
-      (LENGTH : length xs = length ys)
-      (LOOKUP : ∀ i : nat, ∀ x : A, ∀ y : A, (xs !! i = Some x /\ ys !! i = Some y) -> x = y)
-      : xs = ys.
-    Proof.
-      generalize dependent ys. induction xs as [ | x xs IH], ys as [ | y ys]; simpl; intros; try congruence. f_equal.
-      - eapply LOOKUP with (i := 0%nat); simpl; tauto.
-      - eapply IH. { word. }
-        intros i x1 y1 [H_x1 H_y1]. eapply LOOKUP with (i := S i); simpl; tauto.
-    Qed.
+  Lemma list_ext (xs : list A) (ys : list A)
+    (LENGTH : length xs = length ys)
+    (LOOKUP : ∀ i : nat, ∀ x : A, ∀ y : A, (xs !! i = Some x /\ ys !! i = Some y) -> x = y)
+    : xs = ys.
+  Proof.
+    generalize dependent ys. induction xs as [ | x xs IH], ys as [ | y ys]; simpl; intros; try congruence. f_equal.
+    - eapply LOOKUP with (i := 0%nat); simpl; tauto.
+    - eapply IH. { word. }
+      intros i x1 y1 [H_x1 H_y1]. eapply LOOKUP with (i := S i); simpl; tauto.
+  Qed.
 
-    Lemma rev_app (l1 : list A) (l2 : list A)
-      : rev (l1 ++ l2) = (rev l2 ++ rev l1).
-    Proof.
-      induction l1 as [ | x1 l1 IH]; simpl.
-      - rewrite app_nil_r. reflexivity.
-      - rewrite IH. now rewrite <- app_assoc.
-    Qed.
+  Lemma rev_app (l1 : list A) (l2 : list A)
+    : rev (l1 ++ l2) = (rev l2 ++ rev l1).
+  Proof.
+    induction l1 as [ | x1 l1 IH]; simpl.
+    - rewrite app_nil_r. reflexivity.
+    - rewrite IH. now rewrite <- app_assoc.
+  Qed.
 
-    Lemma rev_dual (P : list A -> Prop)
-      (DUAL : ∀ l : list A, P (rev l))
-      : ∀ l : list A, P l.
-    Proof.
-      induction l as [ | x l _] using rev_ind.
-      - eapply DUAL with (l := []).
-      - rewrite <- rev_involutive with (l := l). eapply DUAL with (l := (x :: rev l)).
-    Qed.
+  Lemma rev_dual (P : list A -> Prop)
+    (DUAL : ∀ l : list A, P (rev l))
+    : ∀ l : list A, P l.
+  Proof.
+    induction l as [ | x l _] using rev_ind.
+    - eapply DUAL with (l := []).
+    - rewrite <- rev_involutive with (l := l). eapply DUAL with (l := (x :: rev l)).
+  Qed.
 
-    Lemma rev_inj (l1 : list A) (l2 : list A)
-      (EQ : rev l1 = rev l2)
-      : l1 = l2.
-    Proof.
-      rewrite <- rev_involutive with (l := l1). rewrite <- rev_involutive with (l := l2). congruence.
-    Qed.
+  Lemma rev_inj (l1 : list A) (l2 : list A)
+    (EQ : rev l1 = rev l2)
+    : l1 = l2.
+  Proof.
+    rewrite <- rev_involutive with (l := l1). rewrite <- rev_involutive with (l := l2). congruence.
+  Qed.
 
-    Lemma list_rev_ind (P : list A -> Prop)
-      (NIL : P [])
-      (TAIL : forall x, forall xs, P xs -> P (xs ++ [x]))
-      : forall xs, P xs.
-    Proof.
-      intros xs'. rewrite <- rev_involutive with (l := xs').
-      generalize (rev xs') as xs. clear xs'.
-      induction xs as [ | x xs IH]; simpl.
-      - exact NIL.
-      - eapply TAIL. exact IH.
-    Qed.
+  Lemma list_rev_ind (P : list A -> Prop)
+    (NIL : P [])
+    (TAIL : forall x, forall xs, P xs -> P (xs ++ [x]))
+    : forall xs, P xs.
+  Proof.
+    intros xs'. rewrite <- rev_involutive with (l := xs').
+    generalize (rev xs') as xs. clear xs'.
+    induction xs as [ | x xs IH]; simpl.
+    - exact NIL.
+    - eapply TAIL. exact IH.
+  Qed.
 
-    Lemma app_cancel_l (prefix : list A) (suffix1 : list A) (suffix2 : list A)
-      (EQ : prefix ++ suffix1 = prefix ++ suffix2)
-      : suffix1 = suffix2.
-    Proof.
-      revert suffix1 suffix2 EQ; induction prefix as [ | x xs IH]; simpl; intros; eauto. eapply IH; congruence.
-    Qed.
+  Lemma app_cancel_l (prefix : list A) (suffix1 : list A) (suffix2 : list A)
+    (EQ : prefix ++ suffix1 = prefix ++ suffix2)
+    : suffix1 = suffix2.
+  Proof.
+    revert suffix1 suffix2 EQ; induction prefix as [ | x xs IH]; simpl; intros; eauto. eapply IH; congruence.
+  Qed.
 
-    Lemma app_cancel_r (prefix1 : list A) (prefix2 : list A) (suffix : list A)
-      (EQ : prefix1 ++ suffix = prefix2 ++ suffix)
-      : prefix1 = prefix2.
-    Proof.
-      revert prefix1 prefix2 EQ. induction suffix as [suffix] using rev_dual.
-      induction prefix1 as [prefix1] using rev_dual. induction prefix2 as [prefix2] using rev_dual.
-      do 2 rewrite <- rev_app. intros EQ. apply rev_inj in EQ. apply app_cancel_l in EQ. congruence.
-    Qed.
+  Lemma app_cancel_r (prefix1 : list A) (prefix2 : list A) (suffix : list A)
+    (EQ : prefix1 ++ suffix = prefix2 ++ suffix)
+    : prefix1 = prefix2.
+  Proof.
+    revert prefix1 prefix2 EQ. induction suffix as [suffix] using rev_dual.
+    induction prefix1 as [prefix1] using rev_dual. induction prefix2 as [prefix2] using rev_dual.
+    do 2 rewrite <- rev_app. intros EQ. apply rev_inj in EQ. apply app_cancel_l in EQ. congruence.
+  Qed.
 
-    Lemma forallb_spec (p : A -> bool) (xs : list A)
-      : forall b, forallb p xs = b <-> (if b then forall x, In x xs -> p x = true else exists x, In x xs /\ p x = false).
-    Proof with try now firstorder.
-      intros [ | ]; [exact (forallb_forall p xs) | induction xs as [ | x xs IH]; simpl in *]...
-      rewrite andb_false_iff; firstorder; subst...
-    Qed.
+  Lemma forallb_spec (p : A -> bool) (xs : list A)
+    : forall b, forallb p xs = b <-> (if b then forall x, In x xs -> p x = true else exists x, In x xs /\ p x = false).
+  Proof with try now firstorder.
+    intros [ | ]; [exact (forallb_forall p xs) | induction xs as [ | x xs IH]; simpl in *]...
+    rewrite andb_false_iff; firstorder; subst...
+  Qed.
 
-    Lemma In_lookup (xs : list A) (x : A)
-      (IN : In x xs)
-      : exists n : nat, xs !! n = Some x /\ (n < length xs)%nat.
-    Proof with try (word || done).
-      revert x IN; induction xs as [ | x1 xs IH]; simpl; intros x0 IN... destruct IN as [<- | IN].
-      - exists 0%nat... split...
-      - pose proof (IH x0 IN) as (n & EQ & LE). exists (S n). split...
-    Qed.
+  Lemma In_lookup (xs : list A) (x : A)
+    (IN : In x xs)
+    : exists n : nat, xs !! n = Some x /\ (n < length xs)%nat.
+  Proof with try (word || done).
+    revert x IN; induction xs as [ | x1 xs IH]; simpl; intros x0 IN... destruct IN as [<- | IN].
+    - exists 0%nat... split...
+    - pose proof (IH x0 IN) as (n & EQ & LE). exists (S n). split...
+  Qed.
 
-    Lemma lookup_In (xs : list A) (x : A) (n : nat)
-      (LOOKUP : xs !! n = Some x)
-      : In x xs.
-    Proof with try done.
-      revert xs n x LOOKUP; induction xs as [ | x xs IH]; intros [ | n]; simpl; intros...
-      - left; congruence.
-      - enough (In x0 xs) by now right. eapply IH...
-    Qed.
+  Lemma lookup_In (xs : list A) (x : A) (n : nat)
+    (LOOKUP : xs !! n = Some x)
+    : In x xs.
+  Proof with try done.
+    revert xs n x LOOKUP; induction xs as [ | x xs IH]; intros [ | n]; simpl; intros...
+    - left; congruence.
+    - enough (In x0 xs) by now right. eapply IH...
+  Qed.
 
-    Lemma lookup_Some (xs : list A) (i : nat)
-      (RANGE : (i < length xs)%nat)
-      : { x : A | xs !! i = Some x }.
-    Proof.
-      revert i RANGE; induction xs as [ | x xs IH].
-      - simpl. intros; exfalso; word.
-      - intros [ | i] ?; simpl in *.
-        + exists x; trivial.
-        + eapply IH; word.
-    Qed.
+  Lemma lookup_Some (xs : list A) (i : nat)
+    (RANGE : (i < length xs)%nat)
+    : { x : A | xs !! i = Some x }.
+  Proof.
+    revert i RANGE; induction xs as [ | x xs IH].
+    - simpl. intros; exfalso; word.
+    - intros [ | i] ?; simpl in *.
+      + exists x; trivial.
+      + eapply IH; word.
+  Qed.
 
-    Lemma snoc_inv_iff (xs1 : list A) (xs2 : list A) (y1 : A) (y2 : A)
-      : xs1 ++ [y1] = xs2 ++ [y2] <-> (xs1 = xs2 /\ y1 = y2).
-    Proof.
-      split.
-      - intros EQ.
-        assert (length xs1 = length xs2) as LENGTH.
-        { enough (length xs1 + 1 = length xs2 + 1)%nat by word. apply f_equal with (f := length) in EQ. do 2 rewrite length_app in EQ; trivial. }
-        assert (y1 = y2) as H_y.
-        { enough (Some y1 = Some y2) by congruence. erewrite <- lookup_snoc with (l := xs1). erewrite <- lookup_snoc with (l := xs2). congruence. }
-        split; trivial. eapply app_cancel_r with (suffix := [y1]). congruence.
-      - intros [? ?]; congruence.
-    Qed.
+  Lemma snoc_inv_iff (xs1 : list A) (xs2 : list A) (y1 : A) (y2 : A)
+    : xs1 ++ [y1] = xs2 ++ [y2] <-> (xs1 = xs2 /\ y1 = y2).
+  Proof.
+    split.
+    - intros EQ.
+      assert (length xs1 = length xs2) as LENGTH.
+      { enough (length xs1 + 1 = length xs2 + 1)%nat by word. apply f_equal with (f := length) in EQ. do 2 rewrite length_app in EQ; trivial. }
+      assert (y1 = y2) as H_y.
+      { enough (Some y1 = Some y2) by congruence. erewrite <- lookup_snoc with (l := xs1). erewrite <- lookup_snoc with (l := xs2). congruence. }
+      split; trivial. eapply app_cancel_r with (suffix := [y1]). congruence.
+    - intros [? ?]; congruence.
+  Qed.
 
-    Inductive subseq : list A -> list A -> Prop :=
-      | subseq_nil
-        : subseq [] []
-      | subseq_snoc xs ys z
-        (SUBSEQ : subseq xs ys)
-        : subseq xs (ys ++ [z])
-      | subseq_skip xs ys z
-        (SUBSEQ : subseq xs ys)
-        : subseq (xs ++ [z]) (ys ++ [z]).
-
-    #[local] Hint Constructors subseq : core.
-
-    Lemma subseq_Forall_Forall (P : A -> Prop) xs ys
+  Inductive subseq : list A -> list A -> Prop :=
+    | subseq_nil
+      : subseq [] []
+    | subseq_snoc xs ys z
       (SUBSEQ : subseq xs ys)
-      (FORALL : Forall P ys)
-      : Forall P xs.
-    Proof.
-      induction SUBSEQ; eauto.
-      - rewrite Forall_app in FORALL. tauto.
-      - rewrite -> Forall_app in FORALL |- *. tauto.
-    Qed.
+      : subseq xs (ys ++ [z])
+    | subseq_skip xs ys z
+      (SUBSEQ : subseq xs ys)
+      : subseq (xs ++ [z]) (ys ++ [z]).
+
+  #[local] Hint Constructors subseq : core.
+
+  Lemma subseq_Forall_Forall (P : A -> Prop) xs ys
+    (SUBSEQ : subseq xs ys)
+    (FORALL : Forall P ys)
+    : Forall P xs.
+  Proof.
+    induction SUBSEQ; eauto.
+    - rewrite Forall_app in FORALL. tauto.
+    - rewrite -> Forall_app in FORALL |- *. tauto.
+  Qed.
 
   End MORE_LIST_LEMMAS.
 
@@ -267,25 +263,25 @@ Module SessionPrelude.
 
   Section hsEq_accessories.
 
-    Context `{hsEq_A : hsEq A}.
+  Context `{hsEq_A : hsEq A}.
 
-    Lemma eqb_comm (x : A) (y : A)
-      (x_wf : well_formed x)
-      (y_wf : well_formed y)
-      : eqb x y = eqb y x.
-    Proof.
-      destruct (eqb y x) as [ | ] eqn: H_OBS; [rewrite eqb_eq in H_OBS | rewrite eqb_neq in H_OBS]; trivial.
-      - rewrite eqb_eq; eauto with *.
-      - rewrite eqb_neq; eauto with *.
-    Qed.
+  Lemma eqb_comm (x : A) (y : A)
+    (x_wf : well_formed x)
+    (y_wf : well_formed y)
+    : eqb x y = eqb y x.
+  Proof.
+    destruct (eqb y x) as [ | ] eqn: H_OBS; [rewrite eqb_eq in H_OBS | rewrite eqb_neq in H_OBS]; trivial.
+    - rewrite eqb_eq; eauto with *.
+    - rewrite eqb_neq; eauto with *.
+  Qed.
 
-    Lemma eqb_obs (b : bool) (x : A) (y : A)
-      (x_wf : well_formed x)
-      (y_wf : well_formed y)
-      : eqb x y = b <-> (if b then eqProp x y else ~ eqProp x y).
-    Proof.
-      destruct b; [eapply eqb_eq | eapply eqb_neq]; trivial.
-    Qed.
+  Lemma eqb_obs (b : bool) (x : A) (y : A)
+    (x_wf : well_formed x)
+    (y_wf : well_formed y)
+    : eqb x y = b <-> (if b then eqProp x y else ~ eqProp x y).
+  Proof.
+    destruct b; [eapply eqb_eq | eapply eqb_neq]; trivial.
+  Qed.
 
   End hsEq_accessories.
 
@@ -422,24 +418,24 @@ Module SessionPrelude.
 
   Section hsOrd_accessories.
 
-    Context `{hsOrd_A : hsOrd A}.
+  Context `{hsOrd_A : hsOrd A}.
 
-    Lemma ltb_ge (x : A) (y : A)
-      (x_wf : well_formed x)
-      (y_wf : well_formed y)
-      : ltb x y = (negb (ltb y x) && negb (eqb x y))%bool.
-    Proof.
-      (destruct (ltb x y) as [ | ] eqn: H_OBS0; [rewrite ltb_lt in H_OBS0 | rewrite ltb_nlt in H_OBS0]);
-      (destruct (ltb y x) as [ | ] eqn: H_OBS1; [rewrite ltb_lt in H_OBS1 | rewrite ltb_nlt in H_OBS1]);
-      (destruct (eqb x y) as [ | ] eqn: H_OBS2; [rewrite eqb_eq in H_OBS2 | rewrite eqb_neq in H_OBS2]);
-      simpl in *; try congruence.
-      - contradiction (ltProp_irreflexivity x y); try done.
-      - contradiction (ltProp_irreflexivity y y).
-        + eapply eqProp_reflexivity; try done.
-        + eapply ltProp_transitivity with (y := x); try done.
-      - contradiction (ltProp_irreflexivity x y); try done.
-      - pose proof (ltProp_trichotomy x y); tauto.
-    Qed.
+  Lemma ltb_ge (x : A) (y : A)
+    (x_wf : well_formed x)
+    (y_wf : well_formed y)
+    : ltb x y = (negb (ltb y x) && negb (eqb x y))%bool.
+  Proof.
+    (destruct (ltb x y) as [ | ] eqn: H_OBS0; [rewrite ltb_lt in H_OBS0 | rewrite ltb_nlt in H_OBS0]);
+    (destruct (ltb y x) as [ | ] eqn: H_OBS1; [rewrite ltb_lt in H_OBS1 | rewrite ltb_nlt in H_OBS1]);
+    (destruct (eqb x y) as [ | ] eqn: H_OBS2; [rewrite eqb_eq in H_OBS2 | rewrite eqb_neq in H_OBS2]);
+    simpl in *; try congruence.
+    - contradiction (ltProp_irreflexivity x y); try done.
+    - contradiction (ltProp_irreflexivity y y).
+      + eapply eqProp_reflexivity; try done.
+      + eapply ltProp_transitivity with (y := x); try done.
+    - contradiction (ltProp_irreflexivity x y); try done.
+    - pose proof (ltProp_trichotomy x y); tauto.
+  Qed.
 
   End hsOrd_accessories.
 
@@ -557,498 +553,498 @@ Module SessionPrelude.
 
   Section SORTED.
 
-    Context {A : Type} {well_formed : A -> Prop}.
+  Context {A : Type} {well_formed : A -> Prop}.
 
-    Lemma Forall_well_formed_elim (xs : list A)
-      (xs_wf : Forall well_formed xs)
-      : ∀ x : A, ∀ i : nat, xs !! i = Some x -> well_formed x.
-    Proof.
-      induction xs_wf as [ | x xs x_wf xs_wf IH]; intros x0 i H_x0.
-      - rewrite lookup_nil in H_x0. congruence.
-      - rewrite lookup_cons in H_x0. destruct i as [ | i'].
-        + congruence.
-        + eapply IH with (i := i'); trivial.
-    Qed.
+  Lemma Forall_well_formed_elim (xs : list A)
+    (xs_wf : Forall well_formed xs)
+    : ∀ x : A, ∀ i : nat, xs !! i = Some x -> well_formed x.
+  Proof.
+    induction xs_wf as [ | x xs x_wf xs_wf IH]; intros x0 i H_x0.
+    - rewrite lookup_nil in H_x0. congruence.
+    - rewrite lookup_cons in H_x0. destruct i as [ | i'].
+      + congruence.
+      + eapply IH with (i := i'); trivial.
+  Qed.
 
-    #[local] Hint Resolve Forall_well_formed_elim : core.
+  #[local] Hint Resolve Forall_well_formed_elim : core.
 
-    Context {hsEq : hsEq A (well_formed := well_formed)}.
+  Context {hsEq : hsEq A (well_formed := well_formed)}.
 
-    Context {hsOrd : hsOrd A (hsEq := hsEq)}.
+  Context {hsOrd : hsOrd A (hsEq := hsEq)}.
 
-    Definition isSorted (xs : list A) : Prop :=
-      ∀ i : nat, ∀ j : nat, (i < j)%nat ->
-      ∀ x1 : A, ∀ x2 : A, xs !! i = Some x1 -> xs !! j = Some x2 -> ltb x1 x2 = true.
+  Definition isSorted (xs : list A) : Prop :=
+    ∀ i : nat, ∀ j : nat, (i < j)%nat ->
+    ∀ x1 : A, ∀ x2 : A, xs !! i = Some x1 -> xs !! j = Some x2 -> ltb x1 x2 = true.
 
-    Lemma isSorted_middle_1 (xs : list A) (y : A) (zs : list A)
-      (SORTED : isSorted (xs ++ y :: zs))
-      : isSorted (xs ++ zs).
-    Proof.
-      intros i j i_lt_j x1 x2 H_x1 H_x2.
-      assert (i < length xs \/ i >= length xs)%nat as [H_i | H_i] by word; assert (j < length xs \/ j >= length xs)%nat as [H_j | H_j] by word.
-      - rewrite lookup_app_l in H_x1; trivial. rewrite lookup_app_l in H_x2; trivial. eapply SORTED with (i := i) (j := j).
-        + word.
-        + rewrite lookup_app_l; trivial.
-        + rewrite lookup_app_l; trivial.
-      - rewrite lookup_app_l in H_x1; trivial. rewrite lookup_app_r in H_x2; trivial. eapply SORTED with (i := i) (j := (j + 1)%nat).
-        + word.
-        + rewrite lookup_app_l; trivial.
-        + replace (j + 1)%nat with (S j) by word. rewrite lookup_app_r.
-          * rewrite lookup_cons. replace (S j - length xs)%nat with (S (j - length xs)%nat); trivial. word.
-          * word.
-      - word.
-      - rewrite lookup_app_r in H_x1; trivial. rewrite lookup_app_r in H_x2; trivial. eapply SORTED with (i := (i + 1)%nat) (j := (j + 1)%nat).
-        + word.
-        + replace (i + 1)%nat with (S i) by word. rewrite lookup_app_r.
-          * rewrite lookup_cons. replace (S i - length xs)%nat with (S (i - length xs)%nat); trivial. word.
-          * word.
-        + replace (j + 1)%nat with (S j) by word. rewrite lookup_app_r.
-          * rewrite lookup_cons. replace (S j - length xs)%nat with (S (j - length xs)%nat); trivial. word.
-          * word.
-    Qed.
+  Lemma isSorted_middle_1 (xs : list A) (y : A) (zs : list A)
+    (SORTED : isSorted (xs ++ y :: zs))
+    : isSorted (xs ++ zs).
+  Proof.
+    intros i j i_lt_j x1 x2 H_x1 H_x2.
+    assert (i < length xs \/ i >= length xs)%nat as [H_i | H_i] by word; assert (j < length xs \/ j >= length xs)%nat as [H_j | H_j] by word.
+    - rewrite lookup_app_l in H_x1; trivial. rewrite lookup_app_l in H_x2; trivial. eapply SORTED with (i := i) (j := j).
+      + word.
+      + rewrite lookup_app_l; trivial.
+      + rewrite lookup_app_l; trivial.
+    - rewrite lookup_app_l in H_x1; trivial. rewrite lookup_app_r in H_x2; trivial. eapply SORTED with (i := i) (j := (j + 1)%nat).
+      + word.
+      + rewrite lookup_app_l; trivial.
+      + replace (j + 1)%nat with (S j) by word. rewrite lookup_app_r.
+        * rewrite lookup_cons. replace (S j - length xs)%nat with (S (j - length xs)%nat); trivial. word.
+        * word.
+    - word.
+    - rewrite lookup_app_r in H_x1; trivial. rewrite lookup_app_r in H_x2; trivial. eapply SORTED with (i := (i + 1)%nat) (j := (j + 1)%nat).
+      + word.
+      + replace (i + 1)%nat with (S i) by word. rewrite lookup_app_r.
+        * rewrite lookup_cons. replace (S i - length xs)%nat with (S (i - length xs)%nat); trivial. word.
+        * word.
+      + replace (j + 1)%nat with (S j) by word. rewrite lookup_app_r.
+        * rewrite lookup_cons. replace (S j - length xs)%nat with (S (j - length xs)%nat); trivial. word.
+        * word.
+  Qed.
 
-    Lemma isSorted_middle (xs : list A) (ys : list A) (zs : list A)
-      (SORTED : isSorted (xs ++ ys ++ zs))
-      : isSorted (xs ++ zs).
-    Proof.
-      revert xs zs SORTED; induction ys as [ | y ys IH]; intros; simpl in *; trivial.
-      eapply IH. eapply isSorted_middle_1. exact SORTED.
-    Qed.
+  Lemma isSorted_middle (xs : list A) (ys : list A) (zs : list A)
+    (SORTED : isSorted (xs ++ ys ++ zs))
+    : isSorted (xs ++ zs).
+  Proof.
+    revert xs zs SORTED; induction ys as [ | y ys IH]; intros; simpl in *; trivial.
+    eapply IH. eapply isSorted_middle_1. exact SORTED.
+  Qed.
 
-    Lemma isSorted_NoDup l (l_wf : Forall well_formed l)
-      (SORTED : isSorted l)
-      : NoDup l.
-    Proof with eauto.
-      induction l_wf as [ | x xs x_wf xs_wf IH]; simpl; econstructor.
-      - intros H_contra. clear IH. induction H_contra; simpl in *.
-        + contradiction (ltProp_irreflexivity x x)...
-          * eapply eqProp_reflexivity...
-          * rewrite <- ltb_lt... eapply SORTED with (i := 0%nat) (j := 1%nat)...
-        + inv xs_wf. enough (isSorted (x :: l))...
-          replace (x :: l) with ([x] ++ l)... replace (x :: y :: l) with ([x] ++ [y] ++ l) in SORTED...
-          eapply isSorted_middle...
-      - eapply IH. replace xs with ([] ++ xs)... replace (x :: xs) with ([] ++ [x] ++ xs) in SORTED...
+  Lemma isSorted_NoDup l (l_wf : Forall well_formed l)
+    (SORTED : isSorted l)
+    : NoDup l.
+  Proof with eauto.
+    induction l_wf as [ | x xs x_wf xs_wf IH]; simpl; econstructor.
+    - intros H_contra. clear IH. induction H_contra; simpl in *.
+      + contradiction (ltProp_irreflexivity x x)...
+        * eapply eqProp_reflexivity...
+        * rewrite <- ltb_lt... eapply SORTED with (i := 0%nat) (j := 1%nat)...
+      + inv xs_wf. enough (isSorted (x :: l))...
+        replace (x :: l) with ([x] ++ l)... replace (x :: y :: l) with ([x] ++ [y] ++ l) in SORTED...
         eapply isSorted_middle...
-    Qed.
+    - eapply IH. replace xs with ([] ++ xs)... replace (x :: xs) with ([] ++ [x] ++ xs) in SORTED...
+      eapply isSorted_middle...
+  Qed.
 
-    Fixpoint sortedInsert (l : list A) (i : A) : list A :=
-      match l with
-      | [] => [i]
-      | h :: t =>
-        if ltb i h then
-          i :: h :: t
-        else if eqb h i then
-          h :: t
-        else
-          h :: sortedInsert t i
-      end.
+  Fixpoint sortedInsert (l : list A) (i : A) : list A :=
+    match l with
+    | [] => [i]
+    | h :: t =>
+      if ltb i h then
+        i :: h :: t
+      else if eqb h i then
+        h :: t
+      else
+        h :: sortedInsert t i
+    end.
 
-    Lemma Forall_sortedInsert (P : A -> Prop) l i
-      (H_l : Forall P l)
-      (H_i : P i)
-      : Forall P (sortedInsert l i).
-    Proof.
-      induction H_l; simpl; eauto. destruct (ltb i x) as [ | ]; eauto. destruct (eqb x i); eauto.
-    Qed.
+  Lemma Forall_sortedInsert (P : A -> Prop) l i
+    (H_l : Forall P l)
+    (H_i : P i)
+    : Forall P (sortedInsert l i).
+  Proof.
+    induction H_l; simpl; eauto. destruct (ltb i x) as [ | ]; eauto. destruct (eqb x i); eauto.
+  Qed.
 
-    Lemma sortedInsert_spec (l : list A) (i : A) (l_wf : Forall well_formed l) (i_wf : well_formed i)
-      (SORTED : isSorted l)
-      (NOT_IN := forallb (fun j => negb (eqb j i)) l)
-      : ∃ prefix, ∃ suffix, l = prefix ++ suffix /\
-        sortedInsert l i = prefix ++ (if NOT_IN then [i] else []) ++ suffix /\
-        (∀ n : nat, ∀ x : A, prefix !! n = Some x -> ltb x i = true) /\
-        (∀ n : nat, ∀ x : A, suffix !! n = Some x -> if NOT_IN then ltb i x = true else ltb i x = true \/ eqb i x = true) /\
-        Forall well_formed (sortedInsert l i).
-    Proof with eauto.
-      remember l as l' eqn: H_l' in NOT_IN. subst NOT_IN. destruct (forallb (λ j : A, negb (hsEq .(eqb) j i)) l') as [ | ] eqn: H_In.
-      - assert (SUBLIST : forall x, In x l -> In x l') by now subst l'.
-        rewrite forallb_spec in H_In. clear H_l'; revert i SORTED i_wf l' SUBLIST H_In.
-        induction l_wf as [ | x1 xs x1_wf xs_wf IH]; intros x0 SORTED' x0_wf l SUBLIST NOT_In; simpl in *.
-        + exists []. exists []. simpl. split. { done. } split. { reflexivity. } split.
-          { intros n x H_x. rewrite lookup_nil in H_x. congruence. } split.
-          { intros n x H_x. rewrite lookup_nil in H_x. congruence. } econstructor...
-        + assert (SORTED : isSorted xs).
-          { intros i j i_lt_j x x' H_x H_x'. eapply SORTED' with (i := S i) (j := S j); try (word || done). }
-          assert (SUBLIST' : forall x, In x xs -> In x l) by now firstorder.
-          assert (NOT_In' : forall x, In x l -> negb (eqb x x0) = true) by now firstorder.
-          specialize (IH x0 SORTED x0_wf l SUBLIST' NOT_In').
-          destruct IH as (prefix & suffix & -> & EQ & H_prefix & H_suffix & H_wf)... simpl.
-          destruct (ltb x0 x1) as [ | ] eqn: H_OBS; [rewrite ltb_lt in H_OBS | rewrite ltb_nlt in H_OBS]...
-          { exists []. exists (x1 :: prefix ++ suffix)%list.
-            enough (WTS : forall n : nat, forall x, (x1 :: prefix ++ suffix) !! n = Some x -> ltb x0 x = true).
-            { repeat (split; try done). econstructor... }
-            intros n x H_x. assert (n = 0 \/ 0 < n)%nat as [-> | LT] by word.
-            - simpl in H_x. assert (x = x1) as -> by congruence. rewrite ltb_lt...
-            - rewrite -> ltb_lt... eapply ltProp_transitivity with (y := x1)... rewrite <- ltb_lt...
-          }
-          destruct (eqb x1 x0) as [ | ] eqn: H_OBS'; rewrite eqb_obs in H_OBS'...
-          { pose proof (NOT_In x1 (SUBLIST x1 (or_introl eq_refl))) as claim1. rewrite negb_true_iff in claim1. rewrite eqb_neq in claim1... contradiction. }
-          { exists (x1 :: prefix)%list. exists suffix. split. { done. } split. { simpl. rewrite EQ. simpl. reflexivity. }
-            assert (WTS : forall n : nat, forall x, suffix !! n = Some x -> ltb x0 x = true) by done.
-            repeat (split; try done)... intros [ | n]; simpl; intros x H_x...
-            assert (x = x1) as -> by congruence. clear H_x.
-            rewrite ltb_lt... pose proof (ltProp_trichotomy x0 x1) as [? | [? | ?]]; try done...
-            contradiction H_OBS'. eapply eqProp_symmetry...
-          }
-      - subst l'. rewrite forallb_spec in H_In. destruct H_In as (x2 & x2_in & EQ). rewrite negb_false_iff in EQ.
-        assert (x2_wf : well_formed x2).
-        { eapply List.Forall_forall... }
-        rewrite eqb_eq in EQ... simpl; revert SORTED i i_wf x2 x2_in x2_wf EQ.
-        induction l_wf as [ | x1 xs x1_wf xs_wf IH]; simpl; intros SORTED' x0 x0_wf x2 x2_in x2_wf EQ.
-        { tauto. }
-        assert (SORTED : isSorted xs).
+  Lemma sortedInsert_spec (l : list A) (i : A) (l_wf : Forall well_formed l) (i_wf : well_formed i)
+    (SORTED : isSorted l)
+    (NOT_IN := forallb (fun j => negb (eqb j i)) l)
+    : ∃ prefix, ∃ suffix, l = prefix ++ suffix /\
+      sortedInsert l i = prefix ++ (if NOT_IN then [i] else []) ++ suffix /\
+      (∀ n : nat, ∀ x : A, prefix !! n = Some x -> ltb x i = true) /\
+      (∀ n : nat, ∀ x : A, suffix !! n = Some x -> if NOT_IN then ltb i x = true else ltb i x = true \/ eqb i x = true) /\
+      Forall well_formed (sortedInsert l i).
+  Proof with eauto.
+    remember l as l' eqn: H_l' in NOT_IN. subst NOT_IN. destruct (forallb (λ j : A, negb (hsEq .(eqb) j i)) l') as [ | ] eqn: H_In.
+    - assert (SUBLIST : forall x, In x l -> In x l') by now subst l'.
+      rewrite forallb_spec in H_In. clear H_l'; revert i SORTED i_wf l' SUBLIST H_In.
+      induction l_wf as [ | x1 xs x1_wf xs_wf IH]; intros x0 SORTED' x0_wf l SUBLIST NOT_In; simpl in *.
+      + exists []. exists []. simpl. split. { done. } split. { reflexivity. } split.
+        { intros n x H_x. rewrite lookup_nil in H_x. congruence. } split.
+        { intros n x H_x. rewrite lookup_nil in H_x. congruence. } econstructor...
+      + assert (SORTED : isSorted xs).
         { intros i j i_lt_j x x' H_x H_x'. eapply SORTED' with (i := S i) (j := S j); try (word || done). }
-        destruct x2_in as [<- | x2_in].
-        + replace (eqb x1 x0) with true by now symmetry; eapply eqb_eq; trivial.
-          replace (ltb x0 x1) with false; cycle 1.
-          { symmetry. rewrite ltb_nlt... intros H_contra. eapply (ltProp_irreflexivity x0 x1)... eapply eqProp_symmetry... }
-          exists []. exists (x1 :: xs). simpl. repeat (split; try done)...
+        assert (SUBLIST' : forall x, In x xs -> In x l) by now firstorder.
+        assert (NOT_In' : forall x, In x l -> negb (eqb x x0) = true) by now firstorder.
+        specialize (IH x0 SORTED x0_wf l SUBLIST' NOT_In').
+        destruct IH as (prefix & suffix & -> & EQ & H_prefix & H_suffix & H_wf)... simpl.
+        destruct (ltb x0 x1) as [ | ] eqn: H_OBS; [rewrite ltb_lt in H_OBS | rewrite ltb_nlt in H_OBS]...
+        { exists []. exists (x1 :: prefix ++ suffix)%list.
+          enough (WTS : forall n : nat, forall x, (x1 :: prefix ++ suffix) !! n = Some x -> ltb x0 x = true).
+          { repeat (split; try done). econstructor... }
+          intros n x H_x. assert (n = 0 \/ 0 < n)%nat as [-> | LT] by word.
+          - simpl in H_x. assert (x = x1) as -> by congruence. rewrite ltb_lt...
+          - rewrite -> ltb_lt... eapply ltProp_transitivity with (y := x1)... rewrite <- ltb_lt...
+        }
+        destruct (eqb x1 x0) as [ | ] eqn: H_OBS'; rewrite eqb_obs in H_OBS'...
+        { pose proof (NOT_In x1 (SUBLIST x1 (or_introl eq_refl))) as claim1. rewrite negb_true_iff in claim1. rewrite eqb_neq in claim1... contradiction. }
+        { exists (x1 :: prefix)%list. exists suffix. split. { done. } split. { simpl. rewrite EQ. simpl. reflexivity. }
+          assert (WTS : forall n : nat, forall x, suffix !! n = Some x -> ltb x0 x = true) by done.
+          repeat (split; try done)... intros [ | n]; simpl; intros x H_x...
+          assert (x = x1) as -> by congruence. clear H_x.
+          rewrite ltb_lt... pose proof (ltProp_trichotomy x0 x1) as [? | [? | ?]]; try done...
+          contradiction H_OBS'. eapply eqProp_symmetry...
+        }
+    - subst l'. rewrite forallb_spec in H_In. destruct H_In as (x2 & x2_in & EQ). rewrite negb_false_iff in EQ.
+      assert (x2_wf : well_formed x2).
+      { eapply List.Forall_forall... }
+      rewrite eqb_eq in EQ... simpl; revert SORTED i i_wf x2 x2_in x2_wf EQ.
+      induction l_wf as [ | x1 xs x1_wf xs_wf IH]; simpl; intros SORTED' x0 x0_wf x2 x2_in x2_wf EQ.
+      { tauto. }
+      assert (SORTED : isSorted xs).
+      { intros i j i_lt_j x x' H_x H_x'. eapply SORTED' with (i := S i) (j := S j); try (word || done). }
+      destruct x2_in as [<- | x2_in].
+      + replace (eqb x1 x0) with true by now symmetry; eapply eqb_eq; trivial.
+        replace (ltb x0 x1) with false; cycle 1.
+        { symmetry. rewrite ltb_nlt... intros H_contra. eapply (ltProp_irreflexivity x0 x1)... eapply eqProp_symmetry... }
+        exists []. exists (x1 :: xs). simpl. repeat (split; try done)...
+        intros [ | n]; simpl; intros x H_x.
+        * assert (x = x1) as -> by congruence. clear H_x.
+          rewrite ltb_lt... rewrite eqb_eq... pose proof (ltProp_trichotomy x0 x1) as [? | [? | ?]]; try done...
+          contradiction (ltProp_irreflexivity x1 x0)...
+        * assert (claim1 : ltb x1 x = true).
+          { eapply SORTED' with (i := 0%nat) (j := S n); try (word || done). }
+          rewrite ltb_lt in claim1... rewrite ltb_lt... rewrite eqb_eq...
+          pose proof (ltProp_trichotomy x0 x) as [? | [? | ?]]...
+          contradiction (ltProp_irreflexivity x1 x0)... eapply ltProp_transitivity with (y := x)...
+      + destruct (ltb x0 x1) as [ | ] eqn: H_OBS1; [rewrite ltb_lt in H_OBS1 | rewrite ltb_nlt in H_OBS1]...
+        { contradiction (ltProp_irreflexivity x0 x2)...
+          - eapply eqProp_symmetry...
+          - pose proof (In_lookup xs x2 x2_in) as (n & H_OBS & LEN).
+            eapply ltProp_transitivity with (y := x1)... rewrite <- ltb_lt... eapply SORTED' with (i := 0%nat) (j := S n)... word.
+        }
+        destruct (eqb x1 x0) as [ | ] eqn: H_OBS2; [rewrite eqb_eq in H_OBS2 | rewrite eqb_neq in H_OBS2]...
+        { exists []. exists (x1 :: xs). simpl. repeat (split; try done)...
           intros [ | n]; simpl; intros x H_x.
-          * assert (x = x1) as -> by congruence. clear H_x.
+          - assert (x = x1) as -> by congruence. clear H_x.
             rewrite ltb_lt... rewrite eqb_eq... pose proof (ltProp_trichotomy x0 x1) as [? | [? | ?]]; try done...
             contradiction (ltProp_irreflexivity x1 x0)...
-          * assert (claim1 : ltb x1 x = true).
+          - assert (claim1 : ltb x1 x = true).
             { eapply SORTED' with (i := 0%nat) (j := S n); try (word || done). }
             rewrite ltb_lt in claim1... rewrite ltb_lt... rewrite eqb_eq...
             pose proof (ltProp_trichotomy x0 x) as [? | [? | ?]]...
             contradiction (ltProp_irreflexivity x1 x0)... eapply ltProp_transitivity with (y := x)...
-        + destruct (ltb x0 x1) as [ | ] eqn: H_OBS1; [rewrite ltb_lt in H_OBS1 | rewrite ltb_nlt in H_OBS1]...
-          { contradiction (ltProp_irreflexivity x0 x2)...
-            - eapply eqProp_symmetry...
-            - pose proof (In_lookup xs x2 x2_in) as (n & H_OBS & LEN).
-              eapply ltProp_transitivity with (y := x1)... rewrite <- ltb_lt... eapply SORTED' with (i := 0%nat) (j := S n)... word.
-          }
-          destruct (eqb x1 x0) as [ | ] eqn: H_OBS2; [rewrite eqb_eq in H_OBS2 | rewrite eqb_neq in H_OBS2]...
-          { exists []. exists (x1 :: xs). simpl. repeat (split; try done)...
-            intros [ | n]; simpl; intros x H_x.
-            - assert (x = x1) as -> by congruence. clear H_x.
-              rewrite ltb_lt... rewrite eqb_eq... pose proof (ltProp_trichotomy x0 x1) as [? | [? | ?]]; try done...
-              contradiction (ltProp_irreflexivity x1 x0)...
-            - assert (claim1 : ltb x1 x = true).
-              { eapply SORTED' with (i := 0%nat) (j := S n); try (word || done). }
-              rewrite ltb_lt in claim1... rewrite ltb_lt... rewrite eqb_eq...
-              pose proof (ltProp_trichotomy x0 x) as [? | [? | ?]]...
-              contradiction (ltProp_irreflexivity x1 x0)... eapply ltProp_transitivity with (y := x)...
-          }
-          { pose proof (IH SORTED x0 x0_wf x2 x2_in x2_wf EQ) as (prefix & suffix & -> & IH' & H_prefix & H_suffix & WF).
-            exists (x1 :: prefix). exists suffix. simpl. rewrite IH'. repeat (split; try done)...
-            intros [ | n]; simpl; intros x H_x...
-            assert (x = x1) as -> by congruence. clear H_x.
-            rewrite ltb_lt... pose proof (ltProp_trichotomy x1 x0) as [? | [? | ?]]...
-            - contradiction H_OBS2.
-            - contradiction H_OBS1.
-          }
-    Qed.
+        }
+        { pose proof (IH SORTED x0 x0_wf x2 x2_in x2_wf EQ) as (prefix & suffix & -> & IH' & H_prefix & H_suffix & WF).
+          exists (x1 :: prefix). exists suffix. simpl. rewrite IH'. repeat (split; try done)...
+          intros [ | n]; simpl; intros x H_x...
+          assert (x = x1) as -> by congruence. clear H_x.
+          rewrite ltb_lt... pose proof (ltProp_trichotomy x1 x0) as [? | [? | ?]]...
+          - contradiction H_OBS2.
+          - contradiction H_OBS1.
+        }
+  Qed.
 
-    Lemma sortedInsert_unique (l : list A) (i : A) (l_wf : Forall well_formed l) (i_wf : well_formed i) (prefix : list A) (suffix : list A)
-      (SORTED : isSorted l)
-      (NOT_IN := forallb (fun j => negb (eqb j i)) l)
-      (APPEND : l = prefix ++ suffix)
-      (PREFIX : ∀ n : nat, ∀ x : A, prefix !! n = Some x -> ltb x i = true)
-      (SUFFIX : ∀ n : nat, ∀ x : A, suffix !! n = Some x -> if NOT_IN then ltb i x = true else ltb i x = true \/ eqb i x = true)
-      : sortedInsert l i = prefix ++ (if NOT_IN then [i] else []) ++ suffix.
-    Proof.
-      remember l as l' eqn: H_l' in NOT_IN. subst NOT_IN. destruct (forallb (λ j : A, negb (hsEq .(eqb) j i)) l') as [ | ] eqn: H_In.
-      - assert (SUBLIST : forall x, In x l -> In x l') by now subst l'.
-        rewrite forallb_spec in H_In. clear H_l'; revert i SORTED i_wf l' SUBLIST H_In prefix suffix PREFIX SUFFIX APPEND.
-        induction l_wf as [ | x1 xs x1_wf xs_wf IH]; intros x0 ? ? ? ? ? prefix suffix; intros; simpl in *.
-        + destruct prefix, suffix; simpl in *; try congruence.
-        + destruct (ltb (A := A) x0 x1) as [ | ] eqn: H_ltb; [rewrite ltb_lt in H_ltb | rewrite ltb_nlt in H_ltb]; trivial.
-          { destruct prefix as [ | x2 xs2].
-            - simpl in *. congruence.
-            - pose proof (PREFIX 0%nat x2 eq_refl) as claim1. pose proof (SUBLIST x1 (or_introl eq_refl)) as claim2.
-              assert (head (x1 :: xs) = head ((x2 :: xs2) ++ suffix)) as claim3 by now f_equal. simpl in claim3. assert (x1 = x2) as <- by congruence.
-              contradiction (ltProp_irreflexivity x1 x1); trivial; [eapply eqProp_reflexivity | eapply ltProp_transitivity with (y := x0)]; trivial. rewrite ltb_lt in claim1; trivial.
-          }
-          destruct (eqb x1 x0) as [ | ] eqn: H_eqb.
-          { rewrite <- negb_false_iff in H_eqb. rewrite H_In in H_eqb; try congruence. eapply SUBLIST. now left. }
-          { rewrite eqb_neq in H_eqb; trivial. destruct prefix as [ | x2 xs2]; simpl in *.
-            - assert (claim1 : ltb x0 x1 = true). { eapply SUFFIX with (n := 0%nat). now rewrite <- APPEND. }
-              rewrite ltb_lt in claim1; trivial. contradiction H_ltb.
-            - assert (x1 = x2) as <- by congruence. f_equal. eapply IH; eauto; try congruence.
-              + eapply isSorted_middle_1 with (xs := []); simpl; exact SORTED.
-              + intros n x H_x. eapply PREFIX with (n := S n). simpl; trivial.
-          }
-      - subst l'. simpl in *. rewrite forallb_spec in H_In. destruct H_In as (x & IN & H_EQ). rewrite negb_false_iff in H_EQ.
-        revert i i_wf prefix suffix PREFIX SUFFIX SORTED APPEND x IN H_EQ. induction l_wf as [ | x1 xs x1_wf xs_wf IH]; intros x0 ? prefix suffix; intros; simpl in *; try tauto.
-        destruct (ltb x0 x1) as [ | ] eqn: H_ltb.
-        { destruct IN as [<- | IN].
-          - rewrite ltb_lt in H_ltb; trivial. contradiction (ltProp_irreflexivity x0 x1); trivial. rewrite eqb_eq in H_EQ; trivial. eapply eqProp_symmetry; trivial.
-          - pose proof (proj1 (List.Forall_forall well_formed xs) xs_wf x IN) as x_wf. destruct prefix as [ | x2 xs2].
-            + simpl in *. apply In_lookup in IN. destruct IN as (n & LOOKUP & LT). rewrite eqb_eq in H_EQ; trivial. contradiction (ltProp_irreflexivity x0 x).
-              * eapply eqProp_symmetry; trivial.
-              * rewrite ltb_lt in H_ltb; trivial. eapply ltProp_transitivity with (y := x1); trivial. rewrite <- ltb_lt; trivial. eapply SORTED with (i := 0%nat) (j := S n); trivial. word.
-            + simpl in *. assert (x2 = x1) as -> by congruence. apply f_equal with (f := tail) in APPEND; simpl in *. subst xs.
-              contradiction (ltProp_irreflexivity x1 x1); trivial.
-              * eapply eqProp_reflexivity; trivial.
-              * rewrite ltb_lt in H_ltb; trivial. eapply ltProp_transitivity with (y := x0); trivial. rewrite <- ltb_lt; trivial. eapply PREFIX with (n := 0%nat). reflexivity.
+  Lemma sortedInsert_unique (l : list A) (i : A) (l_wf : Forall well_formed l) (i_wf : well_formed i) (prefix : list A) (suffix : list A)
+    (SORTED : isSorted l)
+    (NOT_IN := forallb (fun j => negb (eqb j i)) l)
+    (APPEND : l = prefix ++ suffix)
+    (PREFIX : ∀ n : nat, ∀ x : A, prefix !! n = Some x -> ltb x i = true)
+    (SUFFIX : ∀ n : nat, ∀ x : A, suffix !! n = Some x -> if NOT_IN then ltb i x = true else ltb i x = true \/ eqb i x = true)
+    : sortedInsert l i = prefix ++ (if NOT_IN then [i] else []) ++ suffix.
+  Proof.
+    remember l as l' eqn: H_l' in NOT_IN. subst NOT_IN. destruct (forallb (λ j : A, negb (hsEq .(eqb) j i)) l') as [ | ] eqn: H_In.
+    - assert (SUBLIST : forall x, In x l -> In x l') by now subst l'.
+      rewrite forallb_spec in H_In. clear H_l'; revert i SORTED i_wf l' SUBLIST H_In prefix suffix PREFIX SUFFIX APPEND.
+      induction l_wf as [ | x1 xs x1_wf xs_wf IH]; intros x0 ? ? ? ? ? prefix suffix; intros; simpl in *.
+      + destruct prefix, suffix; simpl in *; try congruence.
+      + destruct (ltb (A := A) x0 x1) as [ | ] eqn: H_ltb; [rewrite ltb_lt in H_ltb | rewrite ltb_nlt in H_ltb]; trivial.
+        { destruct prefix as [ | x2 xs2].
+          - simpl in *. congruence.
+          - pose proof (PREFIX 0%nat x2 eq_refl) as claim1. pose proof (SUBLIST x1 (or_introl eq_refl)) as claim2.
+            assert (head (x1 :: xs) = head ((x2 :: xs2) ++ suffix)) as claim3 by now f_equal. simpl in claim3. assert (x1 = x2) as <- by congruence.
+            contradiction (ltProp_irreflexivity x1 x1); trivial; [eapply eqProp_reflexivity | eapply ltProp_transitivity with (y := x0)]; trivial. rewrite ltb_lt in claim1; trivial.
         }
         destruct (eqb x1 x0) as [ | ] eqn: H_eqb.
-        { trivial. }
-        { destruct prefix as [ | x2 xs2]; simpl in *.
-          - destruct IN as [<- | IN].
-            + congruence.
-            + pose proof (proj1 (List.Forall_forall well_formed xs) xs_wf x IN) as x_wf.
-              apply SessionPrelude.In_lookup in IN. destruct IN as (n & LOOKUP & H_n). rewrite eqb_eq in H_EQ; trivial. contradiction (ltProp_irreflexivity x0 x).
-              * eapply eqProp_symmetry; trivial.
-              * pose proof (ltProp_trichotomy x0 x1 i_wf x1_wf) as [? | [? | ?]].
-                { eapply ltProp_transitivity with (y := x1); trivial. rewrite <- ltb_lt; trivial. eapply SORTED with (i := 0%nat) (j := S n); trivial. word. }
-                { rewrite eqb_neq in H_eqb; trivial. contradiction H_eqb. eapply eqProp_transitivity with (y := x); trivial. eapply eqProp_symmetry; trivial. eapply eqProp_transitivity with (y := x0); trivial. }
-                { rewrite ltb_nlt in H_ltb; trivial. rewrite eqb_neq in H_eqb; trivial. pose proof (SUFFIX 0%nat x1) as claim1. rewrite <- APPEND in claim1. simpl in claim1. specialize (claim1 eq_refl). rewrite ltb_lt in claim1; trivial. rewrite eqb_eq in claim1; trivial. destruct claim1; try tauto. contradiction H_eqb. eapply eqProp_symmetry; trivial. }
-          - destruct IN as [<- | IN].
-            + congruence.
-            + assert (x1 = x2) as <- by congruence. f_equal. eapply IH; eauto; try congruence.
-              * intros n x2 H_x2. eapply PREFIX with (n := S n); trivial.
-              * eapply isSorted_middle_1 with (xs := []). simpl. exact SORTED.
+        { rewrite <- negb_false_iff in H_eqb. rewrite H_In in H_eqb; try congruence. eapply SUBLIST. now left. }
+        { rewrite eqb_neq in H_eqb; trivial. destruct prefix as [ | x2 xs2]; simpl in *.
+          - assert (claim1 : ltb x0 x1 = true). { eapply SUFFIX with (n := 0%nat). now rewrite <- APPEND. }
+            rewrite ltb_lt in claim1; trivial. contradiction H_ltb.
+          - assert (x1 = x2) as <- by congruence. f_equal. eapply IH; eauto; try congruence.
+            + eapply isSorted_middle_1 with (xs := []); simpl; exact SORTED.
+            + intros n x H_x. eapply PREFIX with (n := S n). simpl; trivial.
         }
-    Qed.
-
-    Lemma sortedInsert_isSorted l i (l_wf : Forall well_formed l) (i_wf : well_formed i)
-      (SORTED : isSorted l)
-      : isSorted (sortedInsert l i).
-    Proof with try (word || congruence || eauto || done).
-      pose proof (sortedInsert_spec l i l_wf i_wf SORTED) as (prefix & suffix & H_l & -> & H_prefix & H_suffix & H_wf).
-      rename i into x, l into xs. intros i j LE x1 x2 H_x1 H_x2.
-      destruct (forallb (fun j : A => negb (eqb j x)) xs) as [ | ] eqn: H_OBS; simpl.
-      { assert (i < length prefix \/ i = length prefix \/ i > length prefix)%nat as [i_lt | [i_eq | i_gt]] by word;
-        assert (j < length prefix \/ j = length prefix \/ j > length prefix)%nat as [j_lt | [j_eq | j_gt]] by word.
-        - eapply SORTED with (i := i) (j := j)...
-          + rewrite H_l. rewrite lookup_app_l... rewrite lookup_app_l in H_x1...
-          + rewrite H_l. rewrite lookup_app_l... rewrite lookup_app_l in H_x2...
-        - rewrite list_lookup_middle in H_x2...
-          assert (x = x2) as -> by congruence. clear H_x2.
-          eapply H_prefix. rewrite lookup_app_l in H_x1...
-        - rewrite ltb_lt... eapply ltProp_transitivity with (y := x)...
-          + rewrite <- ltb_lt... eapply H_prefix with (n := i)... rewrite lookup_app_l in H_x1...
-          + rewrite <- ltb_lt... eapply H_suffix with (n := (j - (length prefix + 1))%nat)... rewrite lookup_app_r in H_x2... rewrite lookup_app_r in H_x2; simpl in *...
-            replace (j - (length prefix + 1))%nat with (j - length prefix - 1)%nat by word...
-        - rewrite list_lookup_middle in H_x1...
-        - word.
-        - rewrite list_lookup_middle in H_x1...
-          assert (x = x1) as -> by congruence. clear H_x1. eapply H_suffix. rewrite app_assoc in H_x2. rewrite lookup_app_r in H_x2...
-          rewrite length_app. simpl. word.
-        - word.
-        - word.
-        - eapply SORTED with (i := (i - 1)%nat) (j := (j - 1)%nat)...
-          + rewrite H_l. rewrite lookup_app_r... rewrite app_assoc in H_x1. rewrite lookup_app_r in H_x1; simpl in *.
-            * rewrite length_app in H_x1. simpl in *. replace (i - 1 - length prefix)%nat with (i - (length prefix + 1))%nat by word...
-            * rewrite length_app. simpl...
-          + rewrite H_l. rewrite lookup_app_r... rewrite app_assoc in H_x2. rewrite lookup_app_r in H_x2; simpl in *.
-            * rewrite length_app in H_x2. simpl in *. replace (j - 1 - length prefix)%nat with (j - (length prefix + 1))%nat by word...
-            * rewrite length_app. simpl...
+    - subst l'. simpl in *. rewrite forallb_spec in H_In. destruct H_In as (x & IN & H_EQ). rewrite negb_false_iff in H_EQ.
+      revert i i_wf prefix suffix PREFIX SUFFIX SORTED APPEND x IN H_EQ. induction l_wf as [ | x1 xs x1_wf xs_wf IH]; intros x0 ? prefix suffix; intros; simpl in *; try tauto.
+      destruct (ltb x0 x1) as [ | ] eqn: H_ltb.
+      { destruct IN as [<- | IN].
+        - rewrite ltb_lt in H_ltb; trivial. contradiction (ltProp_irreflexivity x0 x1); trivial. rewrite eqb_eq in H_EQ; trivial. eapply eqProp_symmetry; trivial.
+        - pose proof (proj1 (List.Forall_forall well_formed xs) xs_wf x IN) as x_wf. destruct prefix as [ | x2 xs2].
+          + simpl in *. apply In_lookup in IN. destruct IN as (n & LOOKUP & LT). rewrite eqb_eq in H_EQ; trivial. contradiction (ltProp_irreflexivity x0 x).
+            * eapply eqProp_symmetry; trivial.
+            * rewrite ltb_lt in H_ltb; trivial. eapply ltProp_transitivity with (y := x1); trivial. rewrite <- ltb_lt; trivial. eapply SORTED with (i := 0%nat) (j := S n); trivial. word.
+          + simpl in *. assert (x2 = x1) as -> by congruence. apply f_equal with (f := tail) in APPEND; simpl in *. subst xs.
+            contradiction (ltProp_irreflexivity x1 x1); trivial.
+            * eapply eqProp_reflexivity; trivial.
+            * rewrite ltb_lt in H_ltb; trivial. eapply ltProp_transitivity with (y := x0); trivial. rewrite <- ltb_lt; trivial. eapply PREFIX with (n := 0%nat). reflexivity.
       }
-      { simpl in *; subst xs... }
-    Qed.
+      destruct (eqb x1 x0) as [ | ] eqn: H_eqb.
+      { trivial. }
+      { destruct prefix as [ | x2 xs2]; simpl in *.
+        - destruct IN as [<- | IN].
+          + congruence.
+          + pose proof (proj1 (List.Forall_forall well_formed xs) xs_wf x IN) as x_wf.
+            apply SessionPrelude.In_lookup in IN. destruct IN as (n & LOOKUP & H_n). rewrite eqb_eq in H_EQ; trivial. contradiction (ltProp_irreflexivity x0 x).
+            * eapply eqProp_symmetry; trivial.
+            * pose proof (ltProp_trichotomy x0 x1 i_wf x1_wf) as [? | [? | ?]].
+              { eapply ltProp_transitivity with (y := x1); trivial. rewrite <- ltb_lt; trivial. eapply SORTED with (i := 0%nat) (j := S n); trivial. word. }
+              { rewrite eqb_neq in H_eqb; trivial. contradiction H_eqb. eapply eqProp_transitivity with (y := x); trivial. eapply eqProp_symmetry; trivial. eapply eqProp_transitivity with (y := x0); trivial. }
+              { rewrite ltb_nlt in H_ltb; trivial. rewrite eqb_neq in H_eqb; trivial. pose proof (SUFFIX 0%nat x1) as claim1. rewrite <- APPEND in claim1. simpl in claim1. specialize (claim1 eq_refl). rewrite ltb_lt in claim1; trivial. rewrite eqb_eq in claim1; trivial. destruct claim1; try tauto. contradiction H_eqb. eapply eqProp_symmetry; trivial. }
+        - destruct IN as [<- | IN].
+          + congruence.
+          + assert (x1 = x2) as <- by congruence. f_equal. eapply IH; eauto; try congruence.
+            * intros n x2 H_x2. eapply PREFIX with (n := S n); trivial.
+            * eapply isSorted_middle_1 with (xs := []). simpl. exact SORTED.
+      }
+  Qed.
 
-    Lemma isSorted_snoc_iff (xs : list A) (y : A)
-      : isSorted (xs ++ [y]) <-> (isSorted xs /\ Forall (fun x => ltb x y = true) xs).
-    Proof.
-      split.
-      - intros SORTED. split.
-        + intros i1 i2 LT z1 z2 H_z1 H_z2. eapply SORTED with (i := i1) (j := i2); trivial.
-          * rewrite lookup_app_l; trivial. eapply lookup_lt_is_Some_1. exists z1; trivial.
-          * rewrite lookup_app_l; trivial. eapply lookup_lt_is_Some_1. exists z2; trivial.
-        + rewrite List.Forall_forall. intros z H_z. pose proof (In_lookup xs z H_z) as (i & LOOKUP & H_i).
-          eapply SORTED with (i := i) (j := length xs); trivial.
-          * rewrite lookup_app_l; trivial.
-          * rewrite lookup_snoc; trivial.
-      - intros [SORTED FORALL] i1 i2 LT z1 z2 H_z1 H_z2. rewrite -> lookup_app in H_z1, H_z2.
-        (destruct (i1 <? _)%nat as [ | ] eqn: H_OBS1; [rewrite Nat.ltb_lt in H_OBS1 | rewrite Nat.ltb_nlt in H_OBS1]); (destruct (i2 <? _)%nat as [ | ] eqn: H_OBS2; [rewrite Nat.ltb_lt in H_OBS2 | rewrite Nat.ltb_nlt in H_OBS2]); try word.
-        + eapply SORTED with (i := i1) (j := i2); trivial.
-        + rewrite lookup_one in H_z2. destruct H_z2 as [<- LENGTH]. rewrite List.Forall_forall in FORALL. eapply FORALL. eapply lookup_In; eauto.
-        + rewrite -> lookup_one in H_z1, H_z2. destruct H_z1 as [<- LENGTH1], H_z2 as [<- LENGTH2]; try word.
-    Qed.
+  Lemma sortedInsert_isSorted l i (l_wf : Forall well_formed l) (i_wf : well_formed i)
+    (SORTED : isSorted l)
+    : isSorted (sortedInsert l i).
+  Proof with try (word || congruence || eauto || done).
+    pose proof (sortedInsert_spec l i l_wf i_wf SORTED) as (prefix & suffix & H_l & -> & H_prefix & H_suffix & H_wf).
+    rename i into x, l into xs. intros i j LE x1 x2 H_x1 H_x2.
+    destruct (forallb (fun j : A => negb (eqb j x)) xs) as [ | ] eqn: H_OBS; simpl.
+    { assert (i < length prefix \/ i = length prefix \/ i > length prefix)%nat as [i_lt | [i_eq | i_gt]] by word;
+      assert (j < length prefix \/ j = length prefix \/ j > length prefix)%nat as [j_lt | [j_eq | j_gt]] by word.
+      - eapply SORTED with (i := i) (j := j)...
+        + rewrite H_l. rewrite lookup_app_l... rewrite lookup_app_l in H_x1...
+        + rewrite H_l. rewrite lookup_app_l... rewrite lookup_app_l in H_x2...
+      - rewrite list_lookup_middle in H_x2...
+        assert (x = x2) as -> by congruence. clear H_x2.
+        eapply H_prefix. rewrite lookup_app_l in H_x1...
+      - rewrite ltb_lt... eapply ltProp_transitivity with (y := x)...
+        + rewrite <- ltb_lt... eapply H_prefix with (n := i)... rewrite lookup_app_l in H_x1...
+        + rewrite <- ltb_lt... eapply H_suffix with (n := (j - (length prefix + 1))%nat)... rewrite lookup_app_r in H_x2... rewrite lookup_app_r in H_x2; simpl in *...
+          replace (j - (length prefix + 1))%nat with (j - length prefix - 1)%nat by word...
+      - rewrite list_lookup_middle in H_x1...
+      - word.
+      - rewrite list_lookup_middle in H_x1...
+        assert (x = x1) as -> by congruence. clear H_x1. eapply H_suffix. rewrite app_assoc in H_x2. rewrite lookup_app_r in H_x2...
+        rewrite length_app. simpl. word.
+      - word.
+      - word.
+      - eapply SORTED with (i := (i - 1)%nat) (j := (j - 1)%nat)...
+        + rewrite H_l. rewrite lookup_app_r... rewrite app_assoc in H_x1. rewrite lookup_app_r in H_x1; simpl in *.
+          * rewrite length_app in H_x1. simpl in *. replace (i - 1 - length prefix)%nat with (i - (length prefix + 1))%nat by word...
+          * rewrite length_app. simpl...
+        + rewrite H_l. rewrite lookup_app_r... rewrite app_assoc in H_x2. rewrite lookup_app_r in H_x2; simpl in *.
+          * rewrite length_app in H_x2. simpl in *. replace (j - 1 - length prefix)%nat with (j - (length prefix + 1))%nat by word...
+          * rewrite length_app. simpl...
+    }
+    { simpl in *; subst xs... }
+  Qed.
 
-    Theorem subseq_isSorted_isSorted xs ys
-      (SUBSEQ : subseq xs ys)
-      (SORTED : isSorted ys)
-      : isSorted xs.
-    Proof.
-      induction SUBSEQ; trivial.
-      - rewrite isSorted_snoc_iff in SORTED. tauto.
-      - rewrite isSorted_snoc_iff in SORTED. rewrite isSorted_snoc_iff. split; try tauto.
-        eapply subseq_Forall_Forall with (ys := ys); try tauto.
-    Qed.
+  Lemma isSorted_snoc_iff (xs : list A) (y : A)
+    : isSorted (xs ++ [y]) <-> (isSorted xs /\ Forall (fun x => ltb x y = true) xs).
+  Proof.
+    split.
+    - intros SORTED. split.
+      + intros i1 i2 LT z1 z2 H_z1 H_z2. eapply SORTED with (i := i1) (j := i2); trivial.
+        * rewrite lookup_app_l; trivial. eapply lookup_lt_is_Some_1. exists z1; trivial.
+        * rewrite lookup_app_l; trivial. eapply lookup_lt_is_Some_1. exists z2; trivial.
+      + rewrite List.Forall_forall. intros z H_z. pose proof (In_lookup xs z H_z) as (i & LOOKUP & H_i).
+        eapply SORTED with (i := i) (j := length xs); trivial.
+        * rewrite lookup_app_l; trivial.
+        * rewrite lookup_snoc; trivial.
+    - intros [SORTED FORALL] i1 i2 LT z1 z2 H_z1 H_z2. rewrite -> lookup_app in H_z1, H_z2.
+      (destruct (i1 <? _)%nat as [ | ] eqn: H_OBS1; [rewrite Nat.ltb_lt in H_OBS1 | rewrite Nat.ltb_nlt in H_OBS1]); (destruct (i2 <? _)%nat as [ | ] eqn: H_OBS2; [rewrite Nat.ltb_lt in H_OBS2 | rewrite Nat.ltb_nlt in H_OBS2]); try word.
+      + eapply SORTED with (i := i1) (j := i2); trivial.
+      + rewrite lookup_one in H_z2. destruct H_z2 as [<- LENGTH]. rewrite List.Forall_forall in FORALL. eapply FORALL. eapply lookup_In; eauto.
+      + rewrite -> lookup_one in H_z1, H_z2. destruct H_z1 as [<- LENGTH1], H_z2 as [<- LENGTH2]; try word.
+  Qed.
+
+  Theorem subseq_isSorted_isSorted xs ys
+    (SUBSEQ : subseq xs ys)
+    (SORTED : isSorted ys)
+    : isSorted xs.
+  Proof.
+    induction SUBSEQ; trivial.
+    - rewrite isSorted_snoc_iff in SORTED. tauto.
+    - rewrite isSorted_snoc_iff in SORTED. rewrite isSorted_snoc_iff. split; try tauto.
+      eapply subseq_Forall_Forall with (ys := ys); try tauto.
+  Qed.
 
   End SORTED.
 
   Section VECTOR.
 
-    #[local] Open Scope list_scope.
+  #[local] Open Scope list_scope.
 
-    #[local] Notation "x =? y" := (SessionPrelude.eqb x y).
+  #[local] Notation "x =? y" := (SessionPrelude.eqb x y).
 
-    #[local] Notation "x >? y" := (SessionPrelude.ltb y x).
+  #[local] Notation "x >? y" := (SessionPrelude.ltb y x).
 
-    Context {A : Type} {well_formed : A -> Prop}.
+  Context {A : Type} {well_formed : A -> Prop}.
 
-    Definition mk_hint : ∀ xs : list A, Forall well_formed xs -> ∀ x : A, ∀ i : nat, xs !! i = Some x -> well_formed x :=
-      @Forall_well_formed_elim A well_formed.
+  Definition mk_hint : ∀ xs : list A, Forall well_formed xs -> ∀ x : A, ∀ i : nat, xs !! i = Some x -> well_formed x :=
+    @Forall_well_formed_elim A well_formed.
 
-    #[local] Hint Resolve mk_hint : core.
+  #[local] Hint Resolve mk_hint : core.
 
-    Context {hsEq : hsEq A (well_formed := well_formed)}.
+  Context {hsEq : hsEq A (well_formed := well_formed)}.
 
-    Fixpoint vectorEq (v1 : list A) (v2 : list A) : bool :=
-      match v1 with
+  Fixpoint vectorEq (v1 : list A) (v2 : list A) : bool :=
+    match v1 with
+    | [] => true
+    | h1 :: t1 =>
+      match v2 with
       | [] => true
-      | h1 :: t1 =>
-        match v2 with
-        | [] => true
-        | h2 :: t2 => if negb (h1 =? h2) then false else vectorEq t1 t2
-        end
-      end.
+      | h2 :: t2 => if negb (h1 =? h2) then false else vectorEq t1 t2
+      end
+    end.
 
-    #[global, program]
-    Instance hsEq_vector (len : nat) : SessionPrelude.hsEq (list A) (well_formed := fun l => Forall well_formed l /\ length l = len) :=
-      { eqProp xs1 xs2 := ∀ i : nat, (i < len)%nat -> ∀ x1 : A, ∀ x2 : A, xs1 !! i = Some x1 -> xs2 !! i = Some x2 -> eqb x1 x2 = true
-      ; eqb := vectorEq
-      ; eqProp_reflexivity xs1 xs1_wf := _
-      ; eqProp_symmetry xs1 xs2 xs1_wf xs2_wf xs1_eq_xs2 := _
-      ; eqProp_transitivity xs1 xs2 xs3 xs1_wf xs2_wf xs3_wf xs1_eq_xs2 xs2_eq_xs3 := _
-      }.
-    Next Obligation with eauto 2.
-      destruct xs1_wf as [xs1_wf xs1_len].
-      intros i i_bound x1 x2 H_x1 H_x2; simpl in *.
-      replace x1 with x2 by congruence.
-      rewrite eqb_eq... eapply eqProp_reflexivity...
-    Qed.
-    Next Obligation with eauto 2.
-      destruct xs1_wf as [xs1_wf xs1_len], xs2_wf as [xs2_wf xs2_len].
-      intros i i_bound x1 x2 H_x1 H_x2; simpl in *.
-      rewrite eqb_comm...
-    Qed.
-    Next Obligation with eauto 2.
-      destruct xs1_wf as [xs1_wf xs1_len], xs2_wf as [xs2_wf xs2_len], xs3_wf as [xs3_wf xs3_len].
-      intros i i_bound x1 x2 H_x1 H_x2; simpl in *.
-      rewrite <- xs2_len in i_bound.
-      pose proof (list_lookup_lt xs2 i i_bound) as (x3 & H_x3).
-      rewrite eqb_eq... eapply eqProp_transitivity with (y := x3)...
-      - rewrite <- eqb_eq... eapply xs1_eq_xs2 with (i := i)... rewrite <- xs2_len...
-      - rewrite <- eqb_eq... eapply xs2_eq_xs3 with (i := i)... rewrite <- xs2_len...
-    Qed.
-    Next Obligation with eauto 2.
-      destruct x_wf as [x_wf x_len], y_wf as [y_wf y_len]. simpl in *. split.
-      - revert len x_len y y_len y_wf. induction x_wf as [ | hx tx hx_wf tx_wf IH]; intros ? <- [ | hy ty] LEN_EQ y_wf EQ [ | i'] i_bound x1 x2 H_x1 H_x2; simpl in *; try congruence; try word; inv y_wf.
-        + rewrite eqb_eq... destruct (x1 =? x2) as [ | ] eqn: H_OBS; rewrite eqb_obs in H_OBS... all: simpl in *; congruence.
-        + rewrite eqb_eq... destruct (hx =? hy) as [ | ] eqn: H_OBS; rewrite eqb_obs in H_OBS... all: simpl in *; try congruence.
-          rewrite <- eqb_eq... eapply IH with (y := ty) (i := i')... all: try word || done.
-      - revert len x_len y y_len y_wf. induction x_wf as [ | hx tx hx_wf tx_wf IH]; intros ? <- [ | hy ty] LEN_EQ y_wf EQ; simpl in *; try congruence; try word; inv y_wf.
-        destruct (hx =? hy) as [ | ] eqn: H_OBS; rewrite eqb_obs in H_OBS; simpl in *...
-        + eapply IH... all: try (word || done). intros i i_bound x1 x2 H_x1 H_x2.
-          eapply EQ with (i := S i)... word.
-        + contradiction H_OBS. rewrite <- eqb_eq... eapply EQ with (i := 0%nat)... word.
-    Qed.
-    Next Obligation with eauto 2.
-      destruct x_wf as [x_wf x_len], y_wf as [y_wf y_len]. simpl in *. split.
-      - revert len x_len y y_len y_wf. induction x_wf as [ | hx tx hx_wf tx_wf IH]; intros ? <- [ | hy ty] LEN_EQ y_wf NE H_contra; simpl in *; try congruence; try word; inv y_wf.
-        destruct (hx =? hy) as [ | ] eqn: H_OBS; rewrite eqb_obs in H_OBS; simpl in *...
-        + eapply IH with (y := ty)... all: try (word || done). intros i i_bound x1 x2 H_x1 H_x2.
-          eapply H_contra with (i := S i)... word.
-        + contradiction H_OBS. rewrite <- eqb_eq... eapply H_contra with (i := 0%nat)... word.
-      - revert len x_len y y_len y_wf. induction x_wf as [ | hx tx hx_wf tx_wf IH]; intros ? <- [ | hy ty] LEN_EQ y_wf NE; simpl in *; try congruence; try word; inv y_wf.
-        + contradiction NE; word.
-        + destruct (hx =? hy) as [ | ] eqn: H_OBS; rewrite eqb_obs in H_OBS; simpl in *...
-          eapply IH with (y := ty)... all: try (word || done). intros H_contra. contradiction NE.
-          intros [ | i'] i_bound x1 x2 H_x1 H_x2; simpl in *...
-          * rewrite eqb_eq... all: try congruence.
-          * eapply H_contra with (i := i')... word.
-    Qed.
+  #[global, program]
+  Instance hsEq_vector (len : nat) : SessionPrelude.hsEq (list A) (well_formed := fun l => Forall well_formed l /\ length l = len) :=
+    { eqProp xs1 xs2 := ∀ i : nat, (i < len)%nat -> ∀ x1 : A, ∀ x2 : A, xs1 !! i = Some x1 -> xs2 !! i = Some x2 -> eqb x1 x2 = true
+    ; eqb := vectorEq
+    ; eqProp_reflexivity xs1 xs1_wf := _
+    ; eqProp_symmetry xs1 xs2 xs1_wf xs2_wf xs1_eq_xs2 := _
+    ; eqProp_transitivity xs1 xs2 xs3 xs1_wf xs2_wf xs3_wf xs1_eq_xs2 xs2_eq_xs3 := _
+    }.
+  Next Obligation with eauto 2.
+    destruct xs1_wf as [xs1_wf xs1_len].
+    intros i i_bound x1 x2 H_x1 H_x2; simpl in *.
+    replace x1 with x2 by congruence.
+    rewrite eqb_eq... eapply eqProp_reflexivity...
+  Qed.
+  Next Obligation with eauto 2.
+    destruct xs1_wf as [xs1_wf xs1_len], xs2_wf as [xs2_wf xs2_len].
+    intros i i_bound x1 x2 H_x1 H_x2; simpl in *.
+    rewrite eqb_comm...
+  Qed.
+  Next Obligation with eauto 2.
+    destruct xs1_wf as [xs1_wf xs1_len], xs2_wf as [xs2_wf xs2_len], xs3_wf as [xs3_wf xs3_len].
+    intros i i_bound x1 x2 H_x1 H_x2; simpl in *.
+    rewrite <- xs2_len in i_bound.
+    pose proof (list_lookup_lt xs2 i i_bound) as (x3 & H_x3).
+    rewrite eqb_eq... eapply eqProp_transitivity with (y := x3)...
+    - rewrite <- eqb_eq... eapply xs1_eq_xs2 with (i := i)... rewrite <- xs2_len...
+    - rewrite <- eqb_eq... eapply xs2_eq_xs3 with (i := i)... rewrite <- xs2_len...
+  Qed.
+  Next Obligation with eauto 2.
+    destruct x_wf as [x_wf x_len], y_wf as [y_wf y_len]. simpl in *. split.
+    - revert len x_len y y_len y_wf. induction x_wf as [ | hx tx hx_wf tx_wf IH]; intros ? <- [ | hy ty] LEN_EQ y_wf EQ [ | i'] i_bound x1 x2 H_x1 H_x2; simpl in *; try congruence; try word; inv y_wf.
+      + rewrite eqb_eq... destruct (x1 =? x2) as [ | ] eqn: H_OBS; rewrite eqb_obs in H_OBS... all: simpl in *; congruence.
+      + rewrite eqb_eq... destruct (hx =? hy) as [ | ] eqn: H_OBS; rewrite eqb_obs in H_OBS... all: simpl in *; try congruence.
+        rewrite <- eqb_eq... eapply IH with (y := ty) (i := i')... all: try word || done.
+    - revert len x_len y y_len y_wf. induction x_wf as [ | hx tx hx_wf tx_wf IH]; intros ? <- [ | hy ty] LEN_EQ y_wf EQ; simpl in *; try congruence; try word; inv y_wf.
+      destruct (hx =? hy) as [ | ] eqn: H_OBS; rewrite eqb_obs in H_OBS; simpl in *...
+      + eapply IH... all: try (word || done). intros i i_bound x1 x2 H_x1 H_x2.
+        eapply EQ with (i := S i)... word.
+      + contradiction H_OBS. rewrite <- eqb_eq... eapply EQ with (i := 0%nat)... word.
+  Qed.
+  Next Obligation with eauto 2.
+    destruct x_wf as [x_wf x_len], y_wf as [y_wf y_len]. simpl in *. split.
+    - revert len x_len y y_len y_wf. induction x_wf as [ | hx tx hx_wf tx_wf IH]; intros ? <- [ | hy ty] LEN_EQ y_wf NE H_contra; simpl in *; try congruence; try word; inv y_wf.
+      destruct (hx =? hy) as [ | ] eqn: H_OBS; rewrite eqb_obs in H_OBS; simpl in *...
+      + eapply IH with (y := ty)... all: try (word || done). intros i i_bound x1 x2 H_x1 H_x2.
+        eapply H_contra with (i := S i)... word.
+      + contradiction H_OBS. rewrite <- eqb_eq... eapply H_contra with (i := 0%nat)... word.
+    - revert len x_len y y_len y_wf. induction x_wf as [ | hx tx hx_wf tx_wf IH]; intros ? <- [ | hy ty] LEN_EQ y_wf NE; simpl in *; try congruence; try word; inv y_wf.
+      + contradiction NE; word.
+      + destruct (hx =? hy) as [ | ] eqn: H_OBS; rewrite eqb_obs in H_OBS; simpl in *...
+        eapply IH with (y := ty)... all: try (word || done). intros H_contra. contradiction NE.
+        intros [ | i'] i_bound x1 x2 H_x1 H_x2; simpl in *...
+        * rewrite eqb_eq... all: try congruence.
+        * eapply H_contra with (i := i')... word.
+  Qed.
 
-    Context {hsOrd : hsOrd A (hsEq := hsEq)}.
+  Context {hsOrd : hsOrd A (hsEq := hsEq)}.
 
-    Fixpoint vectorGt (v1 : list A) (v2 : list A) : bool :=
-      match v1 with
+  Fixpoint vectorGt (v1 : list A) (v2 : list A) : bool :=
+    match v1 with
+    | [] => false 
+    | h1 :: t1 =>
+      match v2 with
       | [] => false 
-      | h1 :: t1 =>
-        match v2 with
-        | [] => false 
-        | h2 :: t2 => if h1 =? h2 then vectorGt t1 t2 else h1 >? h2
-        end
-      end.
+      | h2 :: t2 => if h1 =? h2 then vectorGt t1 t2 else h1 >? h2
+      end
+    end.
 
-    Lemma vectorGt_transitive l1 l2 l3 (l1_wf : Forall well_formed l1) (l2_wf : Forall well_formed l2) (l3_wf : Forall well_formed l3) :
-      vectorGt l3 l2 = true ->
-      vectorGt l2 l1 = true ->
-      vectorGt l3 l1 = true.
-    Proof with congruence || trivial || eauto 2.
-      revert l1 l3 l1_wf l3_wf; induction l2_wf as [ | x2 l2 x2_wf l2_wf IH]; intros ? ? [ | x1 l1 x1_wf l1_wf] [ | x3 l3 x3_wf l3_wf]; simpl in *...
-      repeat (
-        let H_OBS := fresh "H_OBS" in
-        lazymatch goal with
-        | [ |- context [ (eqb _ _) ] ] => destruct (eqb _ _) as [ | ] eqn: H_OBS; [rewrite eqb_eq in H_OBS | rewrite eqb_neq in H_OBS]; trivial
-        | [ |- context [ (ltb _ _) ] ] => destruct (ltb _ _) as [ | ] eqn: H_OBS; [rewrite ltb_lt in H_OBS | rewrite ltb_nlt in H_OBS]; trivial
-        end
-      ); intros l3_gt_l2 l2_gt_l1...
-      - contradiction H_OBS1. eapply eqProp_transitivity with (y := x2)...
-      - contradiction H_OBS0. eapply eqProp_transitivity with (y := x3)... eapply eqProp_symmetry...
-      - pose proof (ltProp_trichotomy x3 x1) as [? | [? | ?]]; try done.
-        contradiction (ltProp_irreflexivity x3 x2)... eapply ltProp_transitivity with (y := x1)...
-      - contradiction H_OBS. eapply eqProp_transitivity with (y := x1)... eapply eqProp_symmetry...
-      - pose proof (ltProp_trichotomy x3 x1) as [? | [? | ?]]; try done.
-        contradiction (ltProp_irreflexivity x2 x1)... eapply ltProp_transitivity with (y := x3)...
-      - contradiction (ltProp_irreflexivity x1 x3); try done.
-        + eapply eqProp_symmetry...
-        + eapply ltProp_transitivity with (y := x2)...
-      - contradiction H_OBS4. eapply ltProp_transitivity with (y := x2)...
-    Qed.
+  Lemma vectorGt_transitive l1 l2 l3 (l1_wf : Forall well_formed l1) (l2_wf : Forall well_formed l2) (l3_wf : Forall well_formed l3) :
+    vectorGt l3 l2 = true ->
+    vectorGt l2 l1 = true ->
+    vectorGt l3 l1 = true.
+  Proof with congruence || trivial || eauto 2.
+    revert l1 l3 l1_wf l3_wf; induction l2_wf as [ | x2 l2 x2_wf l2_wf IH]; intros ? ? [ | x1 l1 x1_wf l1_wf] [ | x3 l3 x3_wf l3_wf]; simpl in *...
+    repeat (
+      let H_OBS := fresh "H_OBS" in
+      lazymatch goal with
+      | [ |- context [ (eqb _ _) ] ] => destruct (eqb _ _) as [ | ] eqn: H_OBS; [rewrite eqb_eq in H_OBS | rewrite eqb_neq in H_OBS]; trivial
+      | [ |- context [ (ltb _ _) ] ] => destruct (ltb _ _) as [ | ] eqn: H_OBS; [rewrite ltb_lt in H_OBS | rewrite ltb_nlt in H_OBS]; trivial
+      end
+    ); intros l3_gt_l2 l2_gt_l1...
+    - contradiction H_OBS1. eapply eqProp_transitivity with (y := x2)...
+    - contradiction H_OBS0. eapply eqProp_transitivity with (y := x3)... eapply eqProp_symmetry...
+    - pose proof (ltProp_trichotomy x3 x1) as [? | [? | ?]]; try done.
+      contradiction (ltProp_irreflexivity x3 x2)... eapply ltProp_transitivity with (y := x1)...
+    - contradiction H_OBS. eapply eqProp_transitivity with (y := x1)... eapply eqProp_symmetry...
+    - pose proof (ltProp_trichotomy x3 x1) as [? | [? | ?]]; try done.
+      contradiction (ltProp_irreflexivity x2 x1)... eapply ltProp_transitivity with (y := x3)...
+    - contradiction (ltProp_irreflexivity x1 x3); try done.
+      + eapply eqProp_symmetry...
+      + eapply ltProp_transitivity with (y := x2)...
+    - contradiction H_OBS4. eapply ltProp_transitivity with (y := x2)...
+  Qed.
 
-    Lemma vectorGt_implies_not_vectorEq l1 l2 (l1_wf : Forall well_formed l1) (l2_wf : Forall well_formed l2) :
-      vectorGt l1 l2 = true ->
-      vectorEq l1 l2 = false.
-    Proof.
-      revert l2 l2_wf. induction l1_wf as [ | x1 xs1 x1_wf xs1_wf IH]; intros ? [ | x2 xs2 x2_wf xs2_wf]; simpl; intros EQ; try congruence.
-      destruct (x1 =? x2) as [ | ] eqn: H_OBS; [rewrite eqb_eq in H_OBS | rewrite eqb_neq in H_OBS]; trivial; simpl in *.
-      eapply IH; trivial.
-    Qed.
+  Lemma vectorGt_implies_not_vectorEq l1 l2 (l1_wf : Forall well_formed l1) (l2_wf : Forall well_formed l2) :
+    vectorGt l1 l2 = true ->
+    vectorEq l1 l2 = false.
+  Proof.
+    revert l2 l2_wf. induction l1_wf as [ | x1 xs1 x1_wf xs1_wf IH]; intros ? [ | x2 xs2 x2_wf xs2_wf]; simpl; intros EQ; try congruence.
+    destruct (x1 =? x2) as [ | ] eqn: H_OBS; [rewrite eqb_eq in H_OBS | rewrite eqb_neq in H_OBS]; trivial; simpl in *.
+    eapply IH; trivial.
+  Qed.
 
-    Lemma vectorEq_implies_not_vectorGt l1 l2 (l1_wf : Forall well_formed l1) (l2_wf : Forall well_formed l2) :
-      vectorEq l1 l2 = true ->
-      vectorGt l1 l2 = false.
-    Proof.
-      revert l2 l2_wf. induction l1_wf as [ | x1 xs1 x1_wf xs1_wf IH]; intros ? [ | x2 xs2 x2_wf xs2_wf]; simpl; intros EQ; try congruence.
-      destruct (x1 =? x2) as [ | ] eqn: H_OBS; [rewrite eqb_eq in H_OBS | rewrite eqb_neq in H_OBS]; trivial; simpl in *.
-      - eapply IH; trivial.
-      - congruence.
-    Qed.
+  Lemma vectorEq_implies_not_vectorGt l1 l2 (l1_wf : Forall well_formed l1) (l2_wf : Forall well_formed l2) :
+    vectorEq l1 l2 = true ->
+    vectorGt l1 l2 = false.
+  Proof.
+    revert l2 l2_wf. induction l1_wf as [ | x1 xs1 x1_wf xs1_wf IH]; intros ? [ | x2 xs2 x2_wf xs2_wf]; simpl; intros EQ; try congruence.
+    destruct (x1 =? x2) as [ | ] eqn: H_OBS; [rewrite eqb_eq in H_OBS | rewrite eqb_neq in H_OBS]; trivial; simpl in *.
+    - eapply IH; trivial.
+    - congruence.
+  Qed.
 
-    #[global, program]
-    Instance hsOrd_vector (len : nat) : SessionPrelude.hsOrd (list A) (hsEq := hsEq_vector len) :=
-      { ltProp xs1 xs2 := vectorGt xs2 xs1 = true
-      ; ltb xs1 xs2 := vectorGt xs2 xs1
-      }.
-    Next Obligation with eauto 2.
-      simpl in *. destruct x_wf as [x_wf x_len], y_wf as [y_wf y_len].
-      rewrite vectorEq_implies_not_vectorGt...
-      change vectorEq with ( @eqb (list A) _ (hsEq_vector len)).
-      rewrite eqb_comm... rewrite eqb_eq...
-    Qed.
-    Next Obligation with eauto 2.
-      simpl in *. destruct x_wf as [x_wf x_len], y_wf as [y_wf y_len], z_wf as [z_wf z_len].
-      simpl in *. eapply vectorGt_transitive with (l2 := y)...
-    Qed.
-    Next Obligation with eauto 2.
-      simpl in *. destruct x_wf as [x_wf x_len], y_wf as [y_wf y_len]. revert y y_wf y_len. revert len x_len.
-      induction x_wf as [ | hx tx hx_wf tx_wf IH]; intros ? <- ? [ | hy ty hy_wf ty_wf] LEN_EQ; simpl in *; try congruence...
-      - right. left. word.
-      - destruct (hx =? hy) as [ | ] eqn: H_OBS; rewrite eqb_obs in H_OBS; simpl in *...
-        + apply eqProp_symmetry in H_OBS... rewrite <- eqb_eq in H_OBS... rewrite H_OBS. symmetry in LEN_EQ.
-          specialize (IH (length ty) (f_equal Nat.pred LEN_EQ) ty ty_wf eq_refl). destruct IH as [IH | [IH | IH]]; try tauto.
-          right. left. intros [ | i'] i_bound x1 x2 H_x1 H_x2; simpl in *.
-          * rewrite eqb_comm in H_OBS... congruence.
-          * eapply IH with (i := i')... word.
-        + rewrite <- eqb_neq in H_OBS... rewrite eqb_comm in H_OBS... rewrite H_OBS...
-          pose proof (ltProp_trichotomy hy hx) as [H_lt | [H_eq | H_gt]]...
-          * rewrite <- ltb_lt in H_lt... right. right...
-          * rewrite eqb_neq in H_OBS... contradiction H_OBS...
-          * rewrite <- ltb_lt in H_gt...
-    Qed.
-    Next Obligation with eauto 2.
-      simpl. reflexivity.
-    Qed.
-    Next Obligation with eauto 2.
-      simpl in *. destruct (vectorGt y x) as [ | ]; split; intros ?; congruence.
-    Qed.
+  #[global, program]
+  Instance hsOrd_vector (len : nat) : SessionPrelude.hsOrd (list A) (hsEq := hsEq_vector len) :=
+    { ltProp xs1 xs2 := vectorGt xs2 xs1 = true
+    ; ltb xs1 xs2 := vectorGt xs2 xs1
+    }.
+  Next Obligation with eauto 2.
+    simpl in *. destruct x_wf as [x_wf x_len], y_wf as [y_wf y_len].
+    rewrite vectorEq_implies_not_vectorGt...
+    change vectorEq with ( @eqb (list A) _ (hsEq_vector len)).
+    rewrite eqb_comm... rewrite eqb_eq...
+  Qed.
+  Next Obligation with eauto 2.
+    simpl in *. destruct x_wf as [x_wf x_len], y_wf as [y_wf y_len], z_wf as [z_wf z_len].
+    simpl in *. eapply vectorGt_transitive with (l2 := y)...
+  Qed.
+  Next Obligation with eauto 2.
+    simpl in *. destruct x_wf as [x_wf x_len], y_wf as [y_wf y_len]. revert y y_wf y_len. revert len x_len.
+    induction x_wf as [ | hx tx hx_wf tx_wf IH]; intros ? <- ? [ | hy ty hy_wf ty_wf] LEN_EQ; simpl in *; try congruence...
+    - right. left. word.
+    - destruct (hx =? hy) as [ | ] eqn: H_OBS; rewrite eqb_obs in H_OBS; simpl in *...
+      + apply eqProp_symmetry in H_OBS... rewrite <- eqb_eq in H_OBS... rewrite H_OBS. symmetry in LEN_EQ.
+        specialize (IH (length ty) (f_equal Nat.pred LEN_EQ) ty ty_wf eq_refl). destruct IH as [IH | [IH | IH]]; try tauto.
+        right. left. intros [ | i'] i_bound x1 x2 H_x1 H_x2; simpl in *.
+        * rewrite eqb_comm in H_OBS... congruence.
+        * eapply IH with (i := i')... word.
+      + rewrite <- eqb_neq in H_OBS... rewrite eqb_comm in H_OBS... rewrite H_OBS...
+        pose proof (ltProp_trichotomy hy hx) as [H_lt | [H_eq | H_gt]]...
+        * rewrite <- ltb_lt in H_lt... right. right...
+        * rewrite eqb_neq in H_OBS... contradiction H_OBS...
+        * rewrite <- ltb_lt in H_gt...
+  Qed.
+  Next Obligation with eauto 2.
+    simpl. reflexivity.
+  Qed.
+  Next Obligation with eauto 2.
+    simpl in *. destruct (vectorGt y x) as [ | ]; split; intros ?; congruence.
+  Qed.
 
   End VECTOR.
 
